### Answer 6.3.2

**Points:** $A=(1,-1,2)$, $B=(0,-1,3)$, $C=(3,0,2)$.

**Vectors:**
$\mathbf{u} = \overrightarrow{AB} = B - A = (-1, 0, 1)$.
$\mathbf{v} = \overrightarrow{AC} = C - A = (2, 1, 0)$.

**Normal Vector:**
$$ \mathbf{n} = \mathbf{u} \times \mathbf{v} = \begin{vmatrix} \mathbf{i} & \mathbf{j} & \mathbf{k} \\ -1 & 0 & 1 \\ 2 & 1 & 0 \end{vmatrix} = \mathbf{i}(-1) - \mathbf{j}(-2) + \mathbf{k}(-1) = (-1, 2, -1) $$

**Plane Equation:**
Use normal $(-1, 2, -1)$ and point $A(1, -1, 2)$.
$-1(x-1) + 2(y+1) - 1(z-2) = 0$.
$-x + 1 + 2y + 2 - z + 2 = 0$.
$-x + 2y - z + 5 = 0 \implies x - 2y + z = 5$.