### Answer 3.1.14

**Hypothesis:** Replace Axiom 3 (Identity) and 4 (Inverse) with **3':** $0\mathbf{p} = \mathbf{0}$.

**1. Proving Additive Identity (Axiom 3):**
Consider $\mathbf{p} + \mathbf{0}$.
Using 3', $\mathbf{0} = 0\mathbf{p}$.
$\mathbf{p} + 0\mathbf{p} = 1\mathbf{p} + 0\mathbf{p}$ (Scalar identity).
$= (1+0)\mathbf{p}$ (Distributive).
$= 1\mathbf{p} = \mathbf{p}$.
So $\mathbf{p} + \mathbf{0} = \mathbf{p}$. The zero vector defined by 3' acts as the identity.

**2. Proving Additive Inverse (Axiom 4):**
We need to find $\mathbf{x}$ such that $\mathbf{p} + \mathbf{x} = \mathbf{0}$.
Consider $\mathbf{x} = (-1)\mathbf{p}$.
$\mathbf{p} + (-1)\mathbf{p} = 1\mathbf{p} + (-1)\mathbf{p}$
$= (1 + (-1))\mathbf{p}$ (Distributive)
$= 0\mathbf{p}$.
By Axiom 3', $0\mathbf{p} = \mathbf{0}$.
So $(-1)\mathbf{p}$ functions as the additive inverse $-\mathbf{p}$.

**Conclusion:** Axiom 3' is sufficient to derive the standard axioms 3 and 4.