### Answer 7.3.7

**Proof (Schur's Lemma):**
We proceed by induction on $n$.
1.  For $n=1$, $A$ is already triangular.
2.  Assume true for $n-1$. Let $A$ have a real eigenvalue $\lambda_1$ and normalized eigenvector $\mathbf{q}_1$.
3.  Extend $\mathbf{q}_1$ to an orthonormal basis $\{\mathbf{q}_1, \dots, \mathbf{q}_n\}$. Form orthogonal matrix $Q = [\mathbf{q}_1 \mid Q_2]$.
4.  Compute $Q^{-1} A Q = Q^T A Q$.
    The first column is $Q^T A \mathbf{q}_1 = Q^T (\lambda_1 \mathbf{q}_1) = \lambda_1 Q^T \mathbf{q}_1 = \lambda_1 \mathbf{e}_1 = (\lambda_1, 0, \dots, 0)^T$.
    So $Q^T A Q = \begin{bmatrix} \lambda_1 & \mathbf{w}^T \\ \mathbf{0} & A' \end{bmatrix}$.
5.  $A'$ is $(n-1) \times (n-1)$. Since $\det(A-\lambda I) = (\lambda_1 - \lambda)\det(A'-\lambda I)$, the eigenvalues of $A'$ are the remaining eigenvalues of $A$, which are real.
6.  By induction, there exists orthogonal $S'$ such that $S'^{-1} A' S' = T'$ (upper triangular).
7.  Let $S = Q \begin{bmatrix} 1 & 0 \\ 0 & S' \end{bmatrix}$. This is orthogonal.
    $S^{-1} A S$ will be upper triangular.