### Answer 3.6.11

**a. Formula for Standard Powers in terms of Legendre:**
We express $1, x, x^2, x^3$ using $L_0, L_1, L_2, L_3$.
1.  $1 = L_0$.
2.  $x = L_1$.
3.  $L_2 = \frac{1}{2}(3x^2 - 1) \implies 2L_2 = 3x^2 - L_0 \implies x^2 = \frac{2}{3}L_2 + \frac{1}{3}L_0$.
4.  $L_3 = \frac{1}{2}(5x^3 - 3x) \implies 2L_3 = 5x^3 - 3L_1 \implies x^3 = \frac{2}{5}L_3 + \frac{3}{5}L_1$.

**b. Polynomial $P(x) = 1 - 2x + 3x^2 - 4x^3$:**
Substitute the expressions from (a):
$$ P(x) = 1(L_0) - 2(L_1) + 3\left(\frac{2}{3}L_2 + \frac{1}{3}L_0\right) - 4\left(\frac{2}{5}L_3 + \frac{3}{5}L_1\right) $$
$$ = L_0 - 2L_1 + (2L_2 + L_0) - (\frac{8}{5}L_3 + \frac{12}{5}L_1) $$
Group terms:
$L_0$: $1 + 1 = 2$.
$L_1$: $-2 - 2.4 = -4.4$.
$L_2$: $2$.
$L_3$: $-1.6$.
$$ P(x) = 2L_0 - 4.4L_1 + 2L_2 - 1.6L_3 $$