### Answer 3.6.3

**Basis $A$:** $P_A = \begin{bmatrix} 1 & -2 \\ 2 & 1 \end{bmatrix}$.
**Basis $B$:** $P_B = \begin{bmatrix} 3 & 1 \\ 2 & 1 \end{bmatrix}$.

**a. Transition $A \to B$ ($S_{A \to B}$):**
We want $[\mathbf{x}]_B = S [\mathbf{x}]_A$.
We know $\mathbf{x} = P_A [\mathbf{x}]_A$ and $\mathbf{x} = P_B [\mathbf{x}]_B$.
$P_B [\mathbf{x}]_B = P_A [\mathbf{x}]_A \implies [\mathbf{x}]_B = P_B^{-1} P_A [\mathbf{x}]_A$.
So $S = P_B^{-1} P_A$.
$$ P_B^{-1} = \frac{1}{3-2} \begin{bmatrix} 1 & -1 \\ -2 & 3 \end{bmatrix} = \begin{bmatrix} 1 & -1 \\ -2 & 3 \end{bmatrix} $$
$$ S = \begin{bmatrix} 1 & -1 \\ -2 & 3 \end{bmatrix} \begin{bmatrix} 1 & -2 \\ 2 & 1 \end{bmatrix} = \begin{bmatrix} 1-2 & -2-1 \\ -2+6 & 4+3 \end{bmatrix} = \begin{bmatrix} -1 & -3 \\ 4 & 7 \end{bmatrix} $$

**b. $\mathbf{x} = 3\mathbf{b}_1 - 2\mathbf{b}_2$:**
This gives $[\mathbf{x}]_B = (3, -2)^T$. We need $[\mathbf{x}]_A$.
Since $[\mathbf{x}]_B = S [\mathbf{x}]_A$, we solve $S [\mathbf{x}]_A = \begin{bmatrix} 3 \\ -2 \end{bmatrix}$.
Or use $S^{-1}$ (which is $S_{B \to A}$).
$$ S^{-1} = \frac{1}{-7 - (-12)} \begin{bmatrix} 7 & 3 \\ -4 & -1 \end{bmatrix} = \frac{1}{5} \begin{bmatrix} 7 & 3 \\ -4 & -1 \end{bmatrix} $$
$$ [\mathbf{x}]_A = \frac{1}{5} \begin{bmatrix} 7 & 3 \\ -4 & -1 \end{bmatrix} \begin{bmatrix} 3 \\ -2 \end{bmatrix} = \frac{1}{5} \begin{bmatrix} 21-6 \\ -12+2 \end{bmatrix} = \begin{bmatrix} 3 \\ -2 \end{bmatrix} $$
Result: $3\mathbf{a}_1 - 2\mathbf{a}_2$.

**c. $\mathbf{x} = 2\mathbf{a}_1 + 4\mathbf{a}_2$:**
Here $[\mathbf{x}]_A = (2, 4)^T$.
$$ [\mathbf{x}]_B = S [\mathbf{x}]_A = \begin{bmatrix} -1 & -3 \\ 4 & 7 \end{bmatrix} \begin{bmatrix} 2 \\ 4 \end{bmatrix} = \begin{bmatrix} -2-12 \\ 8+28 \end{bmatrix} = \begin{bmatrix} -14 \\ 36 \end{bmatrix} $$
Result: $-14\mathbf{b}_1 + 36\mathbf{b}_2$.