### Answer 3.6.4

**a. Transition $A \to B$:**
$S = P_B^{-1} P_A$.
$$ P_A = \begin{bmatrix} 1 & -2 & 0 \\ 2 & 1 & 0 \\ 0 & 0 & 1 \end{bmatrix}, \quad P_B = \begin{bmatrix} 3 & 1 & 0 \\ 2 & 1 & 0 \\ 0 & 0 & 1 \end{bmatrix} $$
Notice the block structure. The inverse of $P_B$ involves the inverse of the top-left $2 \times 2$ block.
$$ P_B^{-1} = \begin{bmatrix} 1 & -1 & 0 \\ -2 & 3 & 0 \\ 0 & 0 & 1 \end{bmatrix} $$
$$ S = \begin{bmatrix} 1 & -1 & 0 \\ -2 & 3 & 0 \\ 0 & 0 & 1 \end{bmatrix} \begin{bmatrix} 1 & -2 & 0 \\ 2 & 1 & 0 \\ 0 & 0 & 1 \end{bmatrix} = \begin{bmatrix} -1 & -3 & 0 \\ 4 & 7 & 0 \\ 0 & 0 & 1 \end{bmatrix} $$

**b. $\mathbf{x} = 2\mathbf{a}_1 + 4\mathbf{a}_2 + 3\mathbf{a}_3$:**
$[\mathbf{x}]_A = (2, 4, 3)^T$.
$$ [\mathbf{x}]_B = S [\mathbf{x}]_A = \begin{bmatrix} -1 & -3 & 0 \\ 4 & 7 & 0 \\ 0 & 0 & 1 \end{bmatrix} \begin{bmatrix} 2 \\ 4 \\ 3 \end{bmatrix} = \begin{bmatrix} -2-12 \\ 8+28 \\ 3 \end{bmatrix} = \begin{bmatrix} -14 \\ 36 \\ 3 \end{bmatrix} $$
Result: $-14\mathbf{b}_1 + 36\mathbf{b}_2 + 3\mathbf{b}_3$.