**A. Discrete Commutativity:** $(a \star b)[i] = (b \star a)[i]$

1.  **Definition:** $(a \star b)[i] = \sum_{k} a[k] b[i - k]$.

2.  **Substitution:** Let $j = i - k$. Then $k = i - j$.

3.  **Swap:** As $k$ goes from $-\infty$ to $+\infty$, so does $j$.

    $$
    \sum_{j} a[i - j] b[j] = \sum_{j} b[j] a[i - j]
    $$

4.  **Result:** This matches the definition of $(b \star a)[i]$.

**B. Continuous Commutativity:** $(f \star g)(x) = (g \star f)(x)$

1.  **Definition:** $(f \star g)(x) = \int_{-\infty}^{\infty} f(t) g(x - t) dt$.

2.  **Substitution:** Let $u = x - t$, so $t = x - u$ and $dt = -du$.

3.  **Result:**

    $$
    \int_{\infty}^{-\infty} f(x - u) g(u) (-du) = \int_{-\infty}^{\infty} g(u) f(x - u) du
    $$

    This matches $(g \star f)(x)$.

**C. Associativity:** $(a \star (b \star c)) = ((a \star b) \star c)$

- This involves expanding the double sum:

  $$
  (a \star (b \star c))[i] = \sum_j a[j] \left( \sum_k b[k] c[(i-j)-k] \right)
  $$

- By regrouping terms (letting $m = j+k$), you can show this equals the expansion of $((a \star b) \star c)$.
