### Exercise 3.6.4

a. Find the transition matrix $S$ corresponding to the change of basis in $\mathbb{R}^{3}$ from $(\mathbf{a}_{1},\mathbf{a}_{2},\mathbf{a}_{3})$ to $(\mathbf{b}_{1},\mathbf{b}_{2},\mathbf{b}_{3})$, where $\mathbf{a}_{1}=(1,2,0)^{T}$, $\mathbf{a}_{2}=(-2,1,0)^{T}$, $\mathbf{a}_{3}=(0,0,1)^{T}$, $\mathbf{b}_{1}=(3,2,0)^{T}$, $\mathbf{b}_{2}=(1,1,0)^{T}$, $\mathbf{b}_{3}=(0,1,1)^{T}$.

b. Use $S$ to write $\mathbf{x}=2\mathbf{a}_{1}+4\mathbf{a}_{2}+3\mathbf{a}_{3}$ as $x_{B1}\mathbf{b}_{1}+x_{B2}\mathbf{b}_{2}+x_{B3}\mathbf{b}_{3}$.