### Exercise 3.6.3

a. Find the transition matrix $S$ corresponding to the change of basis in $\mathbb{R}^{2}$ from $(\mathbf{a}_{1},\mathbf{a}_{2})$ to $(\mathbf{b}_{1},\mathbf{b}_{2})$, where $\mathbf{a}_{1}=(1,2)^{T}$, $\mathbf{a}_{2}=(-2,1)^{T}$, $\mathbf{b}_{1}=(3,2)^{T}$, $\mathbf{b}_{2}=(1,1)^{T}$.

b. Use $S$ to write $\mathbf{x}=3\mathbf{b}_{1}-2\mathbf{b}_{2}$ as $x_{A1}\mathbf{a}_{1}+x_{A2}\mathbf{a}_{2}$.

c. Use $S$ to write $\mathbf{x}=2\mathbf{a}_{1}+4\mathbf{a}_{2}$ as $x_{B1}\mathbf{b}_{1}+x_{B2}\mathbf{b}_{2}$.