### Answer 4.3

We expand the product $q_1 q_2 = (s_1 + v_1)(s_2 + v_2)$ using the distributive property and quaternion multiplication rules ($i^2=j^2=k^2=-1$, $ij=k$, etc.).

Let $v_1 = x_1 i + y_1 j + z_1 k$ and $v_2 = x_2 i + y_2 j + z_2 k$.

**1. Expand Terms**
$$q_1 q_2 = s_1 s_2 + s_1 v_2 + s_2 v_1 + v_1 v_2$$

**2. Analyze Vector Product $v_1 v_2$**
$$v_1 v_2 = (x_1 i + y_1 j + z_1 k)(x_2 i + y_2 j + z_2 k)$$
$$= x_1 x_2 i^2 + x_1 y_2 ij + x_1 z_2 ik$$
$$+ y_1 x_2 ji + y_1 y_2 j^2 + y_1 z_2 jk$$
$$+ z_1 x_2 ki + z_1 y_2 kj + z_1 z_2 k^2$$

Substitute rules ($i^2=-1, ij=k, ji=-k$, etc.):
$$= -(x_1 x_2 + y_1 y_2 + z_1 z_2)$$
$$+ (y_1 z_2 - z_1 y_2)i + (z_1 x_2 - x_1 z_2)j + (x_1 y_2 - y_1 x_2)k$$

**3. Identify Dot and Cross Products**
Real part: $-(x_1 x_2 + y_1 y_2 + z_1 z_2) = -(v_1 \cdot v_2)$
Imaginary part: $(v_1 \times v_2)$

So, $v_1 v_2 = -v_1 \cdot v_2 + v_1 \times v_2$.

**4. Combine All Parts**
$$q_1 q_2 = s_1 s_2 + s_1 v_2 + s_2 v_1 + (-v_1 \cdot v_2 + v_1 \times v_2)$$
$$q_1 q_2 = s_1 s_2 - v_1 \cdot v_2 + s_1 v_2 + s_2 v_1 + v_1 \times v_2$$
