### Answer 4.4

We seek to prove $(MS) \times (MT) = (\det M)(M^{-1})^T (S \times T)$.

**1. Matrix Representation of Cross Product**
Let $[V]_\times$ be the skew-symmetric matrix such that $[V]_\times U = V \times U$.
The term $(MS) \times (MT)$ can be written as $[MS]_\times MT$.

**2. Relation to Determinant**
For any $3 \times 3$ matrix M and vector S, the property holds:
$$[MS]_\times = (\det M) (M^{-1})^T [S]_\times M^{-1}$$
*(This is a standard identity derived from the fact that $(M S) \times (M T) = Cof(M)(S \times T)$ where $Cof(M) = (\det M)(M^{-1})^T$)*.

**3. Substitute into the expression**
$$(MS) \times (MT) = [MS]_\times (MT)$$
Substitute the identity from step 2:
$$= ((\det M) (M^{-1})^T [S]_\times M^{-1}) (MT)$$
$$= (\det M) (M^{-1})^T [S]_\times (M^{-1} M) T$$
$$= (\det M) (M^{-1})^T [S]_\times I T$$
$$= (\det M) (M^{-1})^T ([S]_\times T)$$

**4. Convert back to Cross Product**
$$= (\det M) (M^{-1})^T (S \times T)$$

Since $S \times T = N$ (the original normal), the transformed normal direction is proportional to $(M^{-1})^T N$.
