### Answer 6.1.4

**Matrix:**
$$ D = \begin{vmatrix} -1 & -2 & 2 & 1 \\ 0 & 0 & -1 & 0 \\ 0 & 0 & 1 & -1 \\ 1 & -1 & 1 & -1 \end{vmatrix} $$

**Row Reduction:**
1.  $R_4 \leftarrow R_4 + R_1$: $(0, -3, 3, 0)$.
    $$ D = \begin{vmatrix} -1 & -2 & 2 & 1 \\ 0 & 0 & -1 & 0 \\ 0 & 0 & 1 & -1 \\ 0 & -3 & 3 & 0 \end{vmatrix} $$
2.  Swap $R_2$ and $R_4$ (Sign change):
    $$ D = - \begin{vmatrix} -1 & -2 & 2 & 1 \\ 0 & -3 & 3 & 0 \\ 0 & 0 & 1 & -1 \\ 0 & 0 & -1 & 0 \end{vmatrix} $$
3.  $R_4 \leftarrow R_4 + R_3$: $(0, 0, 0, -1)$.
    $$ D = - \begin{vmatrix} -1 & -2 & 2 & 1 \\ 0 & -3 & 3 & 0 \\ 0 & 0 & 1 & -1 \\ 0 & 0 & 0 & -1 \end{vmatrix} $$

**Calculation:**
$$ D = - ((-1) \cdot (-3) \cdot 1 \cdot (-1)) = - (-3) = 3 $$