### Answer 6.1.1

**Matrix:**
$$ D = \begin{vmatrix} 2 & -3 & 2 \\ 1 & 4 & 0 \\ 0 & 1 & -5 \end{vmatrix} $$



**Row Reduction:**
1.  Swap $R_1$ and $R_2$ to put a 1 in the pivot (multiply det by $-1$):
    $$ D = (-1) \begin{vmatrix} 1 & 4 & 0 \\ 2 & -3 & 2 \\ 0 & 1 & -5 \end{vmatrix} $$
2.  Eliminate below pivot 1 ($R_2 \leftarrow R_2 - 2R_1$):
    $$ D = (-1) \begin{vmatrix} 1 & 4 & 0 \\ 0 & -11 & 2 \\ 0 & 1 & -5 \end{vmatrix} $$
3.  Swap $R_2$ and $R_3$ (multiply det by $-1$ again, total factor $+1$):
    $$ D = (+1) \begin{vmatrix} 1 & 4 & 0 \\ 0 & 1 & -5 \\ 0 & -11 & 2 \end{vmatrix} $$
4.  Eliminate below pivot 2 ($R_3 \leftarrow R_3 + 11R_2$):
    $$ R_3: (0, -11, 2) + 11(0, 1, -5) = (0, 0, 2 - 55) = (0, 0, -53) $$
    $$ D = \begin{vmatrix} 1 & 4 & 0 \\ 0 & 1 & -5 \\ 0 & 0 & -53 \end{vmatrix} $$

**Calculation:**
The determinant of a triangular matrix is the product of the diagonal entries.
$$ D = 1 \cdot 1 \cdot (-53) = -53 $$