- **Points:** $P_1(1,0,0), P_2(0,1,0), P_3(0,0,1)$.

- **Normal ($\mathbf{n}$):** $(P_2 - P_1) \times (P_3 - P_1) = (-1, 1, 0) \times (-1, 0, 1) = (1, 1, 1)$.

- **Implicit Form:** $(1)x + (1)y + (1)z + D = 0$. Plugging in $(1,0,0)$ gives $D = -1$.

  - Result: $x + y + z - 1 = 0$.

- **Parametric Form:** $P(u, v) = P_1 + u(P_2 - P_1) + v(P_3 - P_1)$.

  - Result: $P(u, v) = (1,0,0) + u(-1,1,0) + v(-1,0,1)$.

- **Normal Vector:** $(1, 1, 1)$ normalized is $(1/\sqrt{3}, 1/\sqrt{3}, 1/\sqrt{3})$.
