- **Goal:** Prove $(a \star b) \star f = a \star (b \star f)$, where $a, b$ are discrete sequences and $f$ is a continuous filter.

- **LHS (Discrete first):** Let $d = a \star b$.

  $$
  d[k] = \sum_j a[j] b[k - j]
  $$

  Now convolve $d$ with $f$ (Reconstruction):

  $$
  (d \star f)(x) = \sum_k d[k] f(x - k) = \sum_k \left( \sum_j a[j] b[k - j] \right) f(x - k)
  $$

- **RHS (Continuous first):** Let $g(x) = (b \star f)(x) = \sum_m b[m] f(x - m)$.
  Now convolve sequence $a$ with continuous signal $g$:

  $$
  (a \star g)(x) = \sum_i a[i] g(x - i) = \sum_i a[i] \left( \sum_m b[m] f((x - i) - m) \right)
  $$

- **Comparison:** By setting $k = i + m$ in the LHS equation, the two summation structures become identical.

- **Result:** The operation is associative, meaning you can pre-convolve the discrete samples or pre-convolve the filter with the samples; the reconstructed signal is the same.
