- **Theorem:** $\mathcal{F} \{ f \star g \} = \hat{f}\hat{g}$

- **Proof:**

  1.  Start with the Fourier definition of the convolution:

      $$
      \mathcal{F} \{ f \star g \} (u) = \int_{-\infty}^{\infty} \left( \int_{-\infty}^{\infty} f(t)g(x-t) dt \right) e^{-2\pi i u x} dx
      $$

  2.  Swap integrals (Fubini's theorem) and group terms:

      $$
      \int_{-\infty}^{\infty} f(t) \left( \int_{-\infty}^{\infty} g(x-t) e^{-2\pi i u x} dx \right) dt
      $$

  3.  Substitute $y = x - t$ (so $x = y + t$) in the inner integral:

      $$
      \int_{-\infty}^{\infty} g(y) e^{-2\pi i u (y+t)} dy = e^{-2\pi i u t} \int_{-\infty}^{\infty} g(y) e^{-2\pi i u y} dy = e^{-2\pi i u t} \hat{g}(u)
      $$

  4.  Substitute back into the outer integral:

      $$
      \int_{-\infty}^{\infty} f(t) e^{-2\pi i u t} \hat{g}(u) dt = \hat{g}(u) \int_{-\infty}^{\infty} f(t) e^{-2\pi i u t} dt
      $$

  5.  **Result:** $\hat{g}(u) \hat{f}(u)$.
