### Answer 1.1.6

**4. If $c\mathbf{p}=\mathbf{0}$, then $c=0$ or $\mathbf{p}=\mathbf{0}$:**
$c\mathbf{p} = (cp_1, \dots, cp_n) = (0, \dots, 0)$.
For each component, $cp_i = 0$. Since these are real numbers, either $c=0$ or $p_i=0$.
If $c \neq 0$, then $p_i$ must be 0 for all $i$, so $\mathbf{p} = \mathbf{0}$.
If $\mathbf{p} \neq \mathbf{0}$, then some $p_k \neq 0$, so $c$ must be 0.

**5. $(-c)\mathbf{p} = c(-\mathbf{p}) = -(c\mathbf{p})$:**
$(-c)\mathbf{p} = (-c p_1, \dots) = -(c p_1, \dots) = -(c\mathbf{p})$.
$c(-\mathbf{p}) = c(-p_1, \dots) = (-c p_1, \dots) = -(c\mathbf{p})$.

**6. $c(\mathbf{p}-\mathbf{q}) = c\mathbf{p} - c\mathbf{q}$:**
$c(\mathbf{p} + (-\mathbf{q})) = c\mathbf{p} + c(-\mathbf{q}) = c\mathbf{p} - c\mathbf{q}$ (using distributive law and part 5).

**7. $(c-d)\mathbf{p} = c\mathbf{p} - d\mathbf{p}$:**
$(c + (-d))\mathbf{p} = c\mathbf{p} + (-d)\mathbf{p} = c\mathbf{p} - d\mathbf{p}$.