### Answer 1.1.3

Given $\mathbf{p}=(2,3,-1)$ and $\mathbf{q}=(1,2,2)$.

**Sum:**
$\mathbf{p} + \mathbf{q} = (2+1, 3+2, -1+2) = (3, 5, 1)$.

**Illustration:**
To illustrate the parallelogram law in 3D:
1.  Draw axes $x, y, z$.
2.  Plot point $P(2,3,-1)$ and draw an arrow from origin $O$ to $P$.
3.  Plot point $Q(1,2,2)$ and draw an arrow from origin $O$ to $Q$.
4.  From the tip of $\mathbf{p}$ ($P$), draw a vector parallel to and with the same length as $\mathbf{q}$. This points to $R(3,5,1)$.
5.  Draw the diagonal arrow from $O$ to $R$. This represents the sum.