### Answer 1.2.2

Given $\mathbf{p} = (2, -2, 1)$ and $\mathbf{q} = (2, 3, 2)$.

1.  **Calculate Squared Lengths:**
    * $|\mathbf{p}|^2 = 2^2 + (-2)^2 + 1^2 = 4+4+1 = 9$
    * $|\mathbf{q}|^2 = 2^2 + 3^2 + 2^2 = 4+9+4 = 17$
    * Sum = $9 + 17 = 26$

2.  **Calculate Sum and Difference Squared Lengths:**
    * $\mathbf{p} + \mathbf{q} = (4, 1, 3) \implies |\mathbf{p}+\mathbf{q}|^2 = 16 + 1 + 9 = 26$
    * $\mathbf{p} - \mathbf{q} = (0, -5, -1) \implies |\mathbf{p}-\mathbf{q}|^2 = 0 + 25 + 1 = 26$

3.  **Conclusion:**
    We see that $|\mathbf{p} \pm \mathbf{q}|^2 = |\mathbf{p}|^2 + |\mathbf{q}|^2$. This is the Pythagorean theorem for vectors.

4.  **Geometric Interpretation:**
    This equality holds if and only if the vectors are **orthogonal** (perpendicular).
    Check dot product: $\mathbf{p} \cdot \mathbf{q} = (2)(2) + (-2)(3) + (1)(2) = 4 - 6 + 2 = 0$.
    Since the dot product is zero, the vectors form a $90^\circ$ angle.