### Answer 5.1.4

**Matrix:** $A = \begin{bmatrix} 1 & 2 \\ 1 & -1 \\ 2 & 1 \end{bmatrix}$. **Vector:** $\mathbf{b} = \begin{bmatrix} 1 \\ -1 \\ 2 \end{bmatrix}$.

**Formula:** Projection $\mathbf{p} = A(A^T A)^{-1} A^T \mathbf{b}$.

1.  **Compute $A^T A$:**
    $$ A^T A = \begin{bmatrix} 1 & 1 & 2 \\ 2 & -1 & 1 \end{bmatrix} \begin{bmatrix} 1 & 2 \\ 1 & -1 \\ 2 & 1 \end{bmatrix} = \begin{bmatrix} 1+1+4 & 2-1+2 \\ 2-1+2 & 4+1+1 \end{bmatrix} = \begin{bmatrix} 6 & 3 \\ 3 & 6 \end{bmatrix} $$

2.  **Compute $(A^T A)^{-1}$:**
    Det $= 36 - 9 = 27$.
    $$ (A^T A)^{-1} = \frac{1}{27} \begin{bmatrix} 6 & -3 \\ -3 & 6 \end{bmatrix} = \frac{1}{9} \begin{bmatrix} 2 & -1 \\ -1 & 2 \end{bmatrix} $$

3.  **Compute $A^T \mathbf{b}$:**
    $$ A^T \mathbf{b} = \begin{bmatrix} 1 & 1 & 2 \\ 2 & -1 & 1 \end{bmatrix} \begin{bmatrix} 1 \\ -1 \\ 2 \end{bmatrix} = \begin{bmatrix} 1 - 1 + 4 \\ 2 + 1 + 2 \end{bmatrix} = \begin{bmatrix} 4 \\ 5 \end{bmatrix} $$

4.  **Compute coefficients $\hat{\mathbf{x}} = (A^T A)^{-1} A^T \mathbf{b}$:**
    $$ \hat{\mathbf{x}} = \frac{1}{9} \begin{bmatrix} 2 & -1 \\ -1 & 2 \end{bmatrix} \begin{bmatrix} 4 \\ 5 \end{bmatrix} = \frac{1}{9} \begin{bmatrix} 8-5 \\ -4+10 \end{bmatrix} = \frac{1}{9} \begin{bmatrix} 3 \\ 6 \end{bmatrix} = \begin{bmatrix} 1/3 \\ 2/3 \end{bmatrix} $$

5.  **Compute Projection $\mathbf{p} = A \hat{\mathbf{x}}$:**
    $$ \mathbf{p} = \begin{bmatrix} 1 & 2 \\ 1 & -1 \\ 2 & 1 \end{bmatrix} \begin{bmatrix} 1/3 \\ 2/3 \end{bmatrix} = \begin{bmatrix} 1/3 + 4/3 \\ 1/3 - 2/3 \\ 2/3 + 2/3 \end{bmatrix} = \begin{bmatrix} 5/3 \\ -1/3 \\ 4/3 \end{bmatrix} $$
