### Answer 3.3

System:
1) $4x + 3y + 2z = 0$
2) $x - y - 3z = 0$
3) $2x + 3y + 4z = 0$

**Gaussian Elimination:**
Swap R1 and R2:
$\begin{bmatrix} 1 & -1 & -3 \\ 4 & 3 & 2 \\ 2 & 3 & 4 \end{bmatrix}$

$R_2 \leftarrow R_2 - 4R_1$: $4 - 4(1) = 0, 3 - 4(-1) = 7, 2 - 4(-3) = 14$
$R_3 \leftarrow R_3 - 2R_1$: $2 - 2(1) = 0, 3 - 2(-1) = 5, 4 - 2(-3) = 10$

Current Matrix:
$\begin{bmatrix} 1 & -1 & -3 \\ 0 & 7 & 14 \\ 0 & 5 & 10 \end{bmatrix}$

Divide R2 by 7; Divide R3 by 5:
$\begin{bmatrix} 1 & -1 & -3 \\ 0 & 1 & 2 \\ 0 & 1 & 2 \end{bmatrix}$

$R_3 \leftarrow R_3 - R_2$:
$\begin{bmatrix} 1 & -1 & -3 \\ 0 & 1 & 2 \\ 0 & 0 & 0 \end{bmatrix}$

**Back Substitution:**
From R2: $y + 2z = 0 \Rightarrow y = -2z$
From R1: $x - y - 3z = 0 \Rightarrow x - (-2z) - 3z = 0 \Rightarrow x - z = 0 \Rightarrow x = z$

**Solution:**
Let $z = t$ (arbitrary parameter).
$$x = t$$
$$y = -2t$$
$$z = t$$
Vector form: $t \langle 1, -2, 1 \rangle$.
