### Answer 3.6

**Proof by Induction:**

**Base Case ($n=1$):**
$\det [a_{11}] = a_{11}$. Holds.

**Inductive Step:**
Assume the determinant of an $(n-1) \times (n-1)$ upper triangular matrix is the product of its diagonal entries.
Consider an $n \times n$ upper triangular matrix M.
Expand the determinant along the first column. Since M is upper triangular, $M_{i1} = 0$ for all $i > 1$.
$$det M = \sum_{i=1}^n (-1)^{i+1} M_{i1} \det M^{\{i,1\}}$$
$$det M = M_{11} \det M^{\{1,1\}} + 0 + ... + 0$$

The minor matrix $M^{\{1,1\}}$ is obtained by removing the first row and first column. The result is an $(n-1) \times (n-1)$ matrix that is still upper triangular, with diagonal entries $M_{22}, M_{33}, ..., M_{nn}$.

By the inductive hypothesis:
$$\det M^{\{1,1\}} = M_{22} M_{33} \cdot ... \cdot M_{nn}$$

Therefore:
$$det M = M_{11} (M_{22} M_{33} \cdot ... \cdot M_{nn})$$
$$det M = \prod_{i=1}^n M_{ii}$$
