### Answer 7.4.9

**Proof:**
Let $q(\mathbf{x}) = \mathbf{x}^H A \mathbf{x}$.
Since $q(\mathbf{x})$ is a scalar (real number), $q(\mathbf{x})^H = \overline{q(\mathbf{x})} = q(\mathbf{x})$.
$q(\mathbf{x})^H = (\mathbf{x}^H A \mathbf{x})^H = \mathbf{x}^H A^H (\mathbf{x}^H)^H = \mathbf{x}^H A^H \mathbf{x}$.
So, $\mathbf{x}^H A \mathbf{x} = \mathbf{x}^H A^H \mathbf{x}$ for all $\mathbf{x}$.
This implies $\mathbf{x}^H (A - A^H) \mathbf{x} = 0$ for all $\mathbf{x}$.
This condition implies $A - A^H = 0 \implies A = A^H$ (Hermitian).
(Note: For complex matrices, $\mathbf{x}^H M \mathbf{x} = 0 \forall \mathbf{x} \implies M=0$. This is not true for real matrices where we only consider real $\mathbf{x}$, but in complex space, it determines the matrix).