### Answer 7.4.16

**Matrix:** $A = \begin{bmatrix} 1 & 1 & 1 \\ 0 & 1 & 1 \\ 0 & -1 & 1 \end{bmatrix}$.

1.  **Eigenvalues:**
    Expand along Col 1: $(1-\lambda) \begin{vmatrix} 1-\lambda & 1 \\ -1 & 1-\lambda \end{vmatrix} = (1-\lambda)((1-\lambda)^2 + 1)$.
    Roots: $\lambda_1 = 1$.
    $(1-\lambda)^2 = -1 \implies \lambda = 1 \pm i$.
    $\lambda_2 = 1-i, \lambda_3 = 1+i$.

2.  **Eigenvectors:**
    * $\lambda = 1$: $(A-I)\mathbf{v}=0 \implies v_2+v_3=0, -v_3=0 \implies v_2=v_3=0$. $v_1$ free. $\mathbf{s}_1 = (1, 0, 0)^T$.
    * $\lambda = 1-i$:
        $\begin{bmatrix} i & 1 & 1 \\ 0 & i & 1 \\ 0 & -1 & i \end{bmatrix} \mathbf{v} = 0$.
        Row 2: $i v_2 + v_3 = 0 \implies v_3 = -i v_2$. Let $v_2 = 1, v_3 = -i$.
        Row 1: $i v_1 + 1 - i = 0 \implies i v_1 = i - 1 \implies v_1 = 1 - 1/i = 1+i$.
        $\mathbf{s}_2 = (1+i, 1, -i)^T$.
    * $\lambda = 1+i$: Conjugate $\mathbf{s}_3 = (1-i, 1, i)^T$.