### Answer 7.4.5

**Given:** $\mathbf{u}_1 = \frac{1}{\sqrt{2}} \begin{bmatrix} 1 \\ i \end{bmatrix}$.

**a. Find $\mathbf{u}_2$:**
We need $\mathbf{u}_2 = \begin{bmatrix} z_1 \\ z_2 \end{bmatrix}$ such that $|\mathbf{u}_2|=1$ and $\mathbf{u}_1^H \mathbf{u}_2 = 0$.
$\frac{1}{\sqrt{2}} [1, -i] \begin{bmatrix} z_1 \\ z_2 \end{bmatrix} = 0 \implies z_1 - iz_2 = 0 \implies z_1 = iz_2$.
Let $z_2 = 1$, then $z_1 = i$. Vector is $\begin{bmatrix} i \\ 1 \end{bmatrix}$.
Norm: $|i|^2 + |1|^2 = 2$. Normalize by dividing by $\sqrt{2}$.
$\mathbf{u}_2 = \frac{1}{\sqrt{2}} \begin{bmatrix} i \\ 1 \end{bmatrix}$.

**b. Coordinates:**
Since the basis is orthonormal, $x_{Uk} = \mathbf{u}_k^H \mathbf{x}$.
$x_{U1} = \mathbf{u}_1^H \mathbf{x} = \frac{1}{\sqrt{2}}(x_1 - ix_2)$.
$x_{U2} = \mathbf{u}_2^H \mathbf{x} = \frac{1}{\sqrt{2}}(-ix_1 + x_2)$.

**c. Specific $\mathbf{x}$:**
$\mathbf{x} = \begin{bmatrix} 2+4i \\ 1-2i \end{bmatrix}$.
$x_{U1} = \frac{1}{\sqrt{2}}((2+4i) - i(1-2i)) = \frac{1}{\sqrt{2}}(2+4i - i - 2) = \frac{3i}{\sqrt{2}}$.
$x_{U2} = \frac{1}{\sqrt{2}}(-i(2+4i) + (1-2i)) = \frac{1}{\sqrt{2}}(-2i + 4 + 1 - 2i) = \frac{5-4i}{\sqrt{2}}$.