### Answer 2.4.14

**Proof of $A^k A^l = A^{k+l}$:**
By definition $A^n$ is $A$ multiplied by itself $n$ times.
$A^k A^l = (\underbrace{A \dots A}_{k}) (\underbrace{A \dots A}_{l}) = \underbrace{A \dots A}_{k+l} = A^{k+l}$.
(Formal proof uses induction on $l$. Base case $l=1$: $A^k A = A^{k+1}$ is definition. Assume true for $l$, show for $l+1$: $A^k A^{l+1} = A^k (A^l A) = (A^k A^l) A = A^{k+l} A = A^{k+l+1}$).

**Proof of $(A^k)^l = A^{kl}$:**
$(A^k)^l = \underbrace{A^k \dots A^k}_{l}$.
Using the first rule repeatedly: $A^k A^k = A^{2k}$, etc.
Sum of exponents is $k + k + \dots + k$ ($l$ times) $= kl$.
Thus $(A^k)^l = A^{kl}$.