### Answer 2.4.9

**Matrices:**
$A = [1 \ -2]$ ($1 \times 2$).
$B = \begin{bmatrix} 3 & -4 \\ 2 & 2 \end{bmatrix}$ ($2 \times 2$).
$C = \begin{bmatrix} 1 & -3 \\ 3 & 0 \end{bmatrix}$ ($2 \times 2$).

**Calculate $(AB)C$:**
$AB = [1(3)-2(2), \ 1(-4)-2(2)] = [3-4, -4-4] = [-1, -8]$.
$(AB)C = [-1, -8] \begin{bmatrix} 1 & -3 \\ 3 & 0 \end{bmatrix}$.
$c_{11} = -1(1) - 8(3) = -1 - 24 = -25$.
$c_{12} = -1(-3) - 8(0) = 3$.
$(AB)C = [-25, \ 3]$.

**Calculate $A(BC)$:**
$BC = \begin{bmatrix} 3(1)-4(3) & 3(-3)-4(0) \\ 2(1)+2(3) & 2(-3)+2(0) \end{bmatrix} = \begin{bmatrix} 3-12 & -9 \\ 2+6 & -6 \end{bmatrix} = \begin{bmatrix} -9 & -9 \\ 8 & -6 \end{bmatrix}$.
$A(BC) = [1 \ -2] \begin{bmatrix} -9 & -9 \\ 8 & -6 \end{bmatrix}$.
$d_{11} = 1(-9) - 2(8) = -9 - 16 = -25$.
$d_{12} = 1(-9) - 2(-6) = -9 + 12 = 3$.
$A(BC) = [-25, \ 3]$.

**Conclusion:**
$(AB)C = A(BC)$. Associative law holds.