### Answer 2.4.3

**Matrices:**
$A = \begin{bmatrix} 1 & -2 & 3 \end{bmatrix}$ ($1 \times 3$)
$B = \begin{bmatrix} 3 \\ 2 \\ 1 \end{bmatrix}$ ($3 \times 1$)

**1. Product $AB$:**
Dimensions: $(1 \times 3) \times (3 \times 1) \to (1 \times 1)$.
$AB = [(1)(3) + (-2)(2) + (3)(1)] = [3 - 4 + 3] = [2]$.

**2. Product $BA$:**
Dimensions: $(3 \times 1) \times (1 \times 3) \to (3 \times 3)$.
$$ BA = \begin{bmatrix} 3 \\ 2 \\ 1 \end{bmatrix} \begin{bmatrix} 1 & -2 & 3 \end{bmatrix} = \begin{bmatrix} (3)(1) & (3)(-2) & (3)(3) \\ (2)(1) & (2)(-2) & (2)(3) \\ (1)(1) & (1)(-2) & (1)(3) \end{bmatrix} = \begin{bmatrix} 3 & -6 & 9 \\ 2 & -4 & 6 \\ 1 & -2 & 3 \end{bmatrix} $$