### Answer 4.3.4

**Vector:** $\mathbf{p} = (x, y, z)$. Let $r = \sqrt{x^2+y^2+z^2}$ and $\rho = \sqrt{x^2+z^2}$.

**a. Rotate about $z$ (to $xz$) then $y$ (to $z$):**
1.  **Rotate about z:** Move $(x,y,z)$ to $(\rho, 0, z)$ (assuming we keep $x > 0$).
    $\cos \theta_1 = x/\sqrt{x^2+y^2}$, $\sin \theta_1 = y/\sqrt{x^2+y^2}$.
    $$ R_z(-\theta_1) = \begin{bmatrix} x/\rho' & y/\rho' & 0 \\ -y/\rho' & x/\rho' & 0 \\ 0 & 0 & 1 \end{bmatrix} \quad (\rho' = \sqrt{x^2+y^2}) $$
2.  **Rotate about y:** Move $(\rho', 0, z)$ to $(0, 0, r)$.
    $\cos \theta_2 = z/r$, $\sin \theta_2 = \rho'/r$.
    We want to rotate $(\rho', z)$ to $(0, r)$. Angle is roughly $90 - \phi$.
    $$ R_y(\theta_2) = \begin{bmatrix} z/r & 0 & -\rho'/r \\ 0 & 1 & 0 \\ \rho'/r & 0 & z/r \end{bmatrix} $$
    Check: $R_y \begin{bmatrix} \rho' \\ 0 \\ z \end{bmatrix} = \begin{bmatrix} (z\rho' - z\rho')/r \\ 0 \\ (\rho'^2 + z^2)/r \end{bmatrix} = \begin{bmatrix} 0 \\ 0 \\ r \end{bmatrix}$. Correct.

**b. Rotate about $z$ (to $yz$) then $x$ (to $z$):**
1.  **Rotate about z:** Move $(x,y,z)$ to $(0, \rho'', z)$ where $\rho'' = \sqrt{x^2+y^2}$.
    $$ R_z(\theta_1) = \begin{bmatrix} y/\rho'' & -x/\rho'' & 0 \\ x/\rho'' & y/\rho'' & 0 \\ 0 & 0 & 1 \end{bmatrix} $$
2.  **Rotate about x:** Move $(0, \rho'', z)$ to $(0, 0, r)$.
    $$ R_x(-\theta_2) = \begin{bmatrix} 1 & 0 & 0 \\ 0 & z/r & -\rho''/r \\ 0 & \rho''/r & z/r \end{bmatrix} $$