### Answer 2.1

Given $P = \langle 2, 2, 1 \rangle$ and $Q = \langle 1, -2, 0 \rangle$.

**(a) Calculate $P \cdot Q$**
$$P \cdot Q = (2)(1) + (2)(-2) + (1)(0)$$
$$= 2 - 4 + 0$$
$$= -2$$
[cite_start][cite: 331, 646]

**(b) Calculate $P \times Q$**
$$P \times Q = \begin{vmatrix} i & j & k \\ 2 & 2 & 1 \\ 1 & -2 & 0 \end{vmatrix}$$
$$= i((2)(0) - (1)(-2)) - j((2)(0) - (1)(1)) + k((2)(-2) - (2)(1))$$
$$= i(0 + 2) - j(0 - 1) + k(-4 - 2)$$
$$= \langle 2, 1, -6 \rangle$$
[cite_start][cite: 433, 434, 647]

**(c) Calculate $proj_P Q$**
The notation $proj_P Q$ refers to the projection of Q onto P.
[cite_start]Formula: $proj_P Q = \frac{Q \cdot P}{||P||^2} P$ [cite: 408]
$$Q \cdot P = -2 \quad \text{(from part a)}$$
$$||P||^2 = 2^2 + 2^2 + 1^2 = 4 + 4 + 1 = 9$$
$$proj_P Q = \frac{-2}{9} \langle 2, 2, 1 \rangle$$
$$= \langle -\frac{4}{9}, -\frac{4}{9}, -\frac{2}{9} \rangle$$
[cite_start][cite: 648]