### Answer 2.2

[cite_start]We apply the Gram-Schmidt process to obtain orthogonal vectors $e'_1, e'_2, e'_3$[cite: 610].

**1. Set $e'_1 = e_1$**
$$e'_1 = \langle \frac{\sqrt{2}}{2}, \frac{\sqrt{2}}{2}, 0 \rangle$$
Note: $||e'_1||^2 = (\frac{\sqrt{2}}{2})^2 + (\frac{\sqrt{2}}{2})^2 = \frac{2}{4} + \frac{2}{4} = 1$.

**2. Calculate $e'_2$**
$$e'_2 = e_2 - \frac{e_2 \cdot e'_1}{||e'_1||^2} e'_1$$
$$e_2 \cdot e'_1 = (-1)(\frac{\sqrt{2}}{2}) + (1)(\frac{\sqrt{2}}{2}) + (-1)(0) = 0$$
Since the dot product is 0, the vectors are already orthogonal.
$$e'_2 = e_2 = \langle -1, 1, -1 \rangle$$
$||e'_2||^2 = (-1)^2 + 1^2 + (-1)^2 = 3$.

**3. Calculate $e'_3$**
$$e'_3 = e_3 - \frac{e_3 \cdot e'_1}{||e'_1||^2} e'_1 - \frac{e_3 \cdot e'_2}{||e'_2||^2} e'_2$$
Compute dot products:
$$e_3 \cdot e'_1 = (0)(\frac{\sqrt{2}}{2}) + (-2)(\frac{\sqrt{2}}{2}) + (-2)(0) = -\sqrt{2}$$
$$e_3 \cdot e'_2 = (0)(-1) + (-2)(1) + (-2)(-1) = -2 + 2 = 0$$
Substitute values:
$$e'_3 = e_3 - \frac{-\sqrt{2}}{1} e'_1 - \frac{0}{3} e'_2$$
$$= \langle 0, -2, -2 \rangle - (-\sqrt{2})\langle \frac{\sqrt{2}}{2}, \frac{\sqrt{2}}{2}, 0 \rangle$$
$$= \langle 0, -2, -2 \rangle + \langle 1, 1, 0 \rangle$$
$$= \langle 1, -1, -2 \rangle$$

**Final Orthogonal Set:**
$$e'_1 = \langle \frac{\sqrt{2}}{2}, \frac{\sqrt{2}}{2}, 0 \rangle$$
$$e'_2 = \langle -1, 1, -1 \rangle$$
$$e'_3 = \langle 1, -1, -2 \rangle$$
[cite_start][cite: 642, 644]