### Answer 2.5

We prove the vector triple product identity for $(P \times Q) \times R$.
Expression to match: $(P \cdot R)Q - (Q \cdot R)P$.
We use the property: $(A \times B) \times C = (A \cdot C)B - (B \cdot C)A$.

**1. Map variables:**
Let $A = P$, $B = Q$, $C = R$.

**2. Apply Formula:**
$$(P \times Q) \times R = (P \cdot R)Q - (Q \cdot R)P$$

**Verification via Component Expansion (x-component):**
Let $S = P \times Q = \langle P_y Q_z - P_z Q_y, P_z Q_x - P_x Q_z, P_x Q_y - P_y Q_x \rangle$.
$$(S \times R)_x = S_y R_z - S_z R_y$$
$$= (P_z Q_x - P_x Q_z)R_z - (P_x Q_y - P_y Q_x)R_y$$
$$= P_z Q_x R_z - P_x Q_z R_z - P_x Q_y R_y + P_y Q_x R_y$$
Add and subtract $P_x Q_x R_x$:
$$= Q_x (P_x R_x + P_y R_y + P_z R_z) - P_x (Q_x R_x + Q_y R_y + Q_z R_z)$$
$$= Q_x (P \cdot R) - P_x (Q \cdot R)$$
This matches the x-component of $(P \cdot R)Q - (Q \cdot R)P$.
[cite_start][cite: 656]