### Answer 2.6

**Part 1: Prove $||P - Q|| \ge ||P|| - ||Q||$**
From the Triangle Inequality, we know:
$$||A + B|| \le ||A|| + [cite_start]||B||$$ [cite: 303]
Let $A = P - Q$ and $B = Q$.
$$||(P - Q) + Q|| \le ||P - Q|| + ||Q||$$
$$||P|| \le ||P - Q|| + ||Q||$$
Subtract $||Q||$ from both sides:
$$||P|| - ||Q|| \le ||P - Q||$$
[cite_start]This proves the inequality[cite: 658].

**Part 2: Extended Triangle Inequality**
We must show $||P|| - ||Q|| \le ||P + Q|| \le ||P|| + ||Q||$.
The right side $||P + Q|| \le ||P|| + [cite_start]||Q||$ is the standard Triangle Inequality[cite: 303].
For the left side, substitute $-Q$ for $Q$ in the inequality proven in Part 1 (since $||-Q|| = ||Q||$):
$$||P - (-Q)|| \ge ||P|| - ||-Q||$$
$$||P + Q|| \ge ||P|| - ||Q||$$
Combining both parts:
$$||P|| - ||Q|| \le ||P + Q|| \le ||P|| + ||Q||$$
[cite_start][cite: 659, 660]