- **Inputs:** $\mathbf{e}=(0,1,0), \mathbf{g}=(0,-1,0), \mathbf{t}=(1,1,0)$.

- **Step 1 (w):** $\mathbf{w}$ points opposite to gaze. $\mathbf{w} = -\mathbf{g} = (0, 1, 0)$ (already normalized).

- **Step 2 (u):** $\mathbf{u} = \mathbf{t} \times \mathbf{w}$.

  - $(1, 1, 0) \times (0, 1, 0) = (0, 0, 1)$.

  - Magnitude is 1, so $\mathbf{u} = (0, 0, 1)$.

- **Step 3 (v):** $\mathbf{v} = \mathbf{w} \times \mathbf{u}$.

  - $(0, 1, 0) \times (0, 0, 1) = (1, 0, 0)$.

- **Result:** Basis is $\mathbf{u}=(0,0,1), \mathbf{v}=(1,0,0), \mathbf{w}=(0,1,0)$.
