### Answer 6.2.3

**Matrix:**
$$ D = \begin{vmatrix} -1 & 1 & 2 & 3 \\ 2 & 0 & -5 & 0 \\ 0 & 0 & 0 & -1 \\ 3 & -3 & 1 & 4 \end{vmatrix} $$

**Expansion along Row 3:**
Only non-zero entry is at $(3, 4)$. Value is $-1$. Sign is $(-1)^{3+4} = -1$.
$$ D = (-1)(-1) \begin{vmatrix} -1 & 1 & 2 \\ 2 & 0 & -5 \\ 3 & -3 & 1 \end{vmatrix} = +1 \cdot D_3 $$
**Calculate $D_3$ (Row 2):**
$2(-1)^{2+1} \begin{vmatrix} 1 & 2 \\ -3 & 1 \end{vmatrix} + 0 + (-5)(-1)^{2+3} \begin{vmatrix} -1 & 1 \\ 3 & -3 \end{vmatrix}$
1.  $-2(1 - (-6)) = -2(7) = -14$.
2.  $+5(3 - 3) = 0$. (Cols dependent, determinant is 0).
Total $D = -14$.