### Answer 6.2.4

**Matrix:**
$$ D = \begin{vmatrix} -1 & -2 & 2 & 1 \\ 0 & 0 & -1 & 0 \\ 0 & 0 & 1 & -1 \\ 1 & -1 & 1 & -1 \end{vmatrix} $$

**Expansion along Row 2:**
Entry $-1$ at $(2,3)$. Sign $(-1)^{2+3} = -1$.
$$ D = (-1)(-1) \begin{vmatrix} -1 & -2 & 1 \\ 0 & 0 & -1 \\ 1 & -1 & -1 \end{vmatrix} = +1 \cdot D' $$
**Calculate $D'$ (Row 2):**
Entry $-1$ at $(2,3)$. Sign $(-1)^{2+3} = -1$.
$$ D' = (-1)(-1) \begin{vmatrix} -1 & -2 \\ 1 & -1 \end{vmatrix} = 1 \cdot (1 - (-2)) = 3 $$
Total $D = 3$.