- **Lagrange Basis Function Formula:**

  $$L_i(x) = \prod_{j=0, j \neq i}^{k} \frac{x - t_j}{t_i - t_j}$$

- **Verification (Example for $i=0$):**

  - Nodes: $t_0=0, t_1=1/3, t_2=2/3, t_3=1$.

  - $L_0(u) = \frac{(u - 1/3)(u - 2/3)(u - 1)}{(0 - 1/3)(0 - 2/3)(0 - 1)} = \frac{u^3 - 2u^2 + 11/9u - 2/9}{-2/9} = -4.5u^3 + 9u^2 - 5.5u + 1$.

- **Conclusion:**

  This polynomial matches the first column of the Basis Matrix found in Exercise 3 (coefficients: $1, -5.5, 9, -4.5$), confirming the result.
