### Answer 2.1.11

**Matrix:**
$$ \left[ \begin{array}{ccccc|c} 3 & -6 & -1 & 1 & 5 & 0 \\ -1 & 2 & 2 & 3 & 3 & 0 \\ 4 & -8 & -3 & -2 & 1 & 0 \end{array} \right] $$

**Elimination:**
1.  Swap $R_1, R_2$, negate: $(1, -2, -2, -3, -3 \mid 0)$.
2.  Eliminate old $R_1$: $R_2 \leftarrow R_2 - 3R_{new}$: $(0, 0, 5, 10, 14 \mid 0)$.
3.  Eliminate old $R_3$: $R_3 \leftarrow R_3 - 4R_{new}$: $(0, 0, 5, 10, 13 \mid 0)$.
    $$ \left[ \begin{array}{ccccc|c} 1 & -2 & -2 & -3 & -3 & 0 \\ 0 & 0 & 5 & 10 & 14 & 0 \\ 0 & 0 & 5 & 10 & 13 & 0 \end{array} \right] $$
4.  $R_3 \leftarrow R_3 - R_2$: $(0, 0, 0, 0, -1 \mid 0)$.

**Back Substitution:**
1.  $-x_5 = 0 \implies x_5 = 0$.
2.  $5x_3 + 10x_4 + 14(0) = 0 \implies x_3 + 2x_4 = 0$.
    $x_4$ is free ($t$). $x_3 = -2t$.
3.  $x_2$ is free ($s$) because the pivot column for $x_2$ is 0.
4.  $x_1 - 2s - 2(-2t) - 3t - 3(0) = 0$.
    $x_1 - 2s + 4t - 3t = 0 \implies x_1 = 2s - t$.

**Solution:**
$$ \mathbf{x} = s(2, 1, 0, 0, 0) + t(-1, 0, -2, 1, 0) $$