### Answer 2.1.10

**Matrix:**
$$ \left[ \begin{array}{ccc|c} 2 & 4 & 1 & 7 \\ 0 & 1 & 3 & 7 \\ 3 & 3 & -1 & 9 \\ 1 & 2 & 3 & 11 \end{array} \right] $$



**Steps:**
1.  Swap $R_1, R_4$ (pivot 1):
    $$ \left[ \begin{array}{ccc|c} 1 & 2 & 3 & 11 \\ 0 & 1 & 3 & 7 \\ 3 & 3 & -1 & 9 \\ 2 & 4 & 1 & 7 \end{array} \right] $$
2.  Eliminate col 1:
    $R_3 \leftarrow R_3 - 3R_1$: $(0, -3, -10 \mid -24)$.
    $R_4 \leftarrow R_4 - 2R_1$: $(0, 0, -5 \mid -15)$.
3.  Eliminate col 2 (pivot at $R_2$ is 1):
    $R_3 \leftarrow R_3 + 3R_2$: $(0, 0, -1 \mid -3)$.
    Matrix:
    $$ \left[ \begin{array}{ccc|c} 1 & 2 & 3 & 11 \\ 0 & 1 & 3 & 7 \\ 0 & 0 & -1 & -3 \\ 0 & 0 & -5 & -15 \end{array} \right] $$
4.  Eliminate col 3:
    $R_4 \leftarrow R_4 - 5R_3$: $(0, 0, 0 \mid 0)$.

**Back Substitution:**
1.  $-x_3 = -3 \implies x_3 = 3$.
2.  $x_2 + 3(3) = 7 \implies x_2 = -2$.
3.  $x_1 + 2(-2) + 3(3) = 11 \implies x_1 - 4 + 9 = 11 \implies x_1 + 5 = 11 \implies x_1 = 6$.

**Solution:**
$$ \mathbf{x} = (6, -2, 3) $$