### Answer 2.1.6

**Matrix:**
$$ \left[ \begin{array}{ccc|c} 1 & 0 & -1 & 1 \\ -2 & 3 & -1 & 0 \\ -6 & 6 & 0 & -2 \end{array} \right] $$

**Elimination:**
1.  $R_2 \leftarrow R_2 + 2R_1$: $(0, 3, -3 \mid 2)$.
2.  $R_3 \leftarrow R_3 + 6R_1$: $(0, 6, -6 \mid 4)$. ($ -2 + 6(1) = 4$).
    $$ \left[ \begin{array}{ccc|c} 1 & 0 & -1 & 1 \\ 0 & 3 & -3 & 2 \\ 0 & 6 & -6 & 4 \end{array} \right] $$
3.  $R_3 \leftarrow R_3 - 2R_2$: LHS zeros out. RHS: $4 - 2(2) = 0$.
    Row of zeros: $0 = 0$. Consistent.

**Back Substitution:**
$x_3 = t$.
$3x_2 - 3t = 2 \implies 3x_2 = 3t + 2 \implies x_2 = t + 2/3$.
$x_1 - t = 1 \implies x_1 = t + 1$.

**Solution:**
$$ \mathbf{x} = \begin{bmatrix} 1 \\ 2/3 \\ 0 \end{bmatrix} + t \begin{bmatrix} 1 \\ 1 \\ 1 \end{bmatrix} $$