### Answer 4.2.3

**Proof:**
($\Rightarrow$) If $T$ is 1-to-1:
$T(\mathbf{x}) = \mathbf{0}$. We know $T(\mathbf{0}) = \mathbf{0}$.
Since $T$ maps distinct vectors to distinct images, $\mathbf{x}$ must be $\mathbf{0}$.
So $Ker(T) = \{\mathbf{0}\}$.

($\Leftarrow$) If $Ker(T) = \{\mathbf{0}\}$:
Assume $T(\mathbf{x}) = T(\mathbf{y})$.
Then $T(\mathbf{x}) - T(\mathbf{y}) = \mathbf{0}$.
$T(\mathbf{x} - \mathbf{y}) = \mathbf{0}$ (Linearity).
So $\mathbf{x} - \mathbf{y} \in Ker(T)$.
Since Kernel is trivial, $\mathbf{x} - \mathbf{y} = \mathbf{0} \implies \mathbf{x} = \mathbf{y}$.
Thus $T$ is 1-to-1.