### Answer 11.1

**(a) Hermite Basis Matrix**
The polynomial $Q(t) = a + bt + ct^2 + dt^3$ must satisfy:
$Q(0) = P_1 \implies a = P_1$
$Q(1) = P_2 \implies a + b + c + d = P_2$
$Q'(0) = T_1 \implies b = T_1$
$Q'(1) = T_2 \implies b + 2c + 3d = T_2$

Substituting $a$ and $b$:
1) $c + d = P_2 - P_1 - T_1$
2) $2c + 3d = T_2 - T_1$

Solving for $c$ and $d$:
From (1): $c = P_2 - P_1 - T_1 - d$. Substitute into (2):
$2(P_2 - P_1 - T_1 - d) + 3d = T_2 - T_1$
$2P_2 - 2P_1 - 2T_1 - 2d + 3d = T_2 - T_1$
$d = -2P_2 + 2P_1 + T_1 + T_2$

Then $c$:
$c = P_2 - P_1 - T_1 - (-2P_2 + 2P_1 + T_1 + T_2)$
$c = 3P_2 - 3P_1 - 2T_1 - T_2$

Coefficients in terms of geometry vector $\begin{bmatrix} P_1 & P_2 & T_1 & T_2 \end{bmatrix}^T$:
$a$: $[1, 0, 0, 0]$
$b$: $[0, 0, 1, 0]$
$c$: $[-3, 3, -2, -1]$
$d$: $[2, -2, 1, 1]$

$$M_{Hermite} = \begin{bmatrix} 2 & -2 & 1 & 1 \\ -3 & 3 & -2 & -1 \\ 0 & 0 & 1 & 0 \\ 1 & 0 & 0 & 0 \end{bmatrix}$$

**(b) BÃ©zier Basis Matrix**
Geometry vector $G_{Bezier} = \begin{bmatrix} P_1 & P_2 & C_1 & C_2 \end{bmatrix}^T$.
Mapping to Hermite geometry $G_{Hermite}$:
$P_1 = P_1$
$P_2 = P_2$
$T_1 = 3(C_1 - P_1)$
$T_2 = 3(P_2 - C_2)$

Transformation $M_{H \to B}$:
$$\begin{bmatrix} P_1 \\ P_2 \\ T_1 \\ T_2 \end{bmatrix} = \begin{bmatrix} 1 & 0 & 0 & 0 \\ 0 & 1 & 0 & 0 \\ -3 & 0 & 3 & 0 \\ 0 & 3 & 0 & -3 \end{bmatrix} \begin{bmatrix} P_1 \\ P_2 \\ C_1 \\ C_2 \end{bmatrix}$$

Multiply $M_{Hermite} \cdot M_{H \to B}$:
$$M_{Bezier} = \begin{bmatrix} 2 & -2 & 1 & 1 \\ -3 & 3 & -2 & -1 \\ 0 & 0 & 1 & 0 \\ 1 & 0 & 0 & 0 \end{bmatrix} \begin{bmatrix} 1 & 0 & 0 & 0 \\ 0 & 1 & 0 & 0 \\ -3 & 0 & 3 & 0 \\ 0 & 3 & 0 & -3 \end{bmatrix} = \begin{bmatrix} -1 & 3 & -3 & 1 \\ 3 & -6 & 3 & 0 \\ -3 & 3 & 0 & 0 \\ 1 & 0 & 0 & 0 \end{bmatrix}$$
