### Answer 11.3

**(a) Sum of Blending Functions**
The KB blending functions are the dot product of the basis matrix $M_{KB}$ and the parameter vector $T(t)$.
For any valid interpolating curve basis (like Hermite based), the sum of the basis functions for the points (rows corresponding to position influence) must effectively sum to 1 to ensure affine invariance (translation of points translates curve).
Specifically, $H_1 + H_2 = 1$ and $H_3 + H_4 = 0$ is not the condition; rather, we check if the sum of weights for $P_{i-1}...P_{i+2}$ is 1.
For the Hermite form $P(t) = (2t^3 - 3t^2 + 1)P_i + (-2t^3 + 3t^2)P_{i+1} + \dots$
The position terms sum to 1. The tangent terms are differences of points.
If $T = c(P_{next} - P_{prev})$, the coefficients of $P$ sum to 0.
Thus, the total sum of coefficients for all $P$ geometry points is $1 + 0 = 1$.

**(b) Continuity Condition**
For $C^1$ continuity, the outgoing tangent of segment $i$ ($T_{out}$) must equal the incoming tangent of segment $i+1$ ($T_{in}$).
$T_{out} = T_{i, 2}$ (Tangent at $P_{i+1}$ for first curve)
$T_{in} = T_{i+1, 1}$ (Tangent at $P_{i+1}$ for second curve)

KB Tangent formulas:
$T_{i,2} = \frac{(1-t)(1-c)(1+b)}{2}(P_{i+1} - P_i) + \frac{(1-t)(1+c)(1-b)}{2}(P_{i+2} - P_{i+1})$
$T_{i+1,1} = \frac{(1-t)(1+c)(1+b)}{2}(P_{i+1} - P_i) + \frac{(1-t)(1-c)(1-b)}{2}(P_{i+2} - P_{i+1})$

For these to be equal for arbitrary $P$, the coefficients must match.
Coeff of $(P_{i+1} - P_i)$: $(1-c)(1+b) = (1+c)(1+b) \implies 1-c = 1+c \implies 2c=0 \implies c=0$.
Coeff of $(P_{i+2} - P_{i+1})$: $(1+c)(1-b) = (1-c)(1-b) \implies 1+c = 1-c \implies c=0$.
**Condition:** The continuity parameter $c$ must be 0 (Canonical spline). $t$ and $b$ can be arbitrary.

**(c) Basis Matrix $M_{KB}$**
Let $s = \frac{1-t}{2}$. (Assuming standard TCB parameters where $c=0$ for simplicity per part b, or generally deriving).
General Tangents at endpoints of segment $P_i, P_{i+1}$:
$T_1 = (1-t)(1+c)(1+b)/2 (P_i - P_{i-1}) + (1-t)(1-c)(1-b)/2 (P_{i+1} - P_i)$
$T_2 = (1-t)(1-c)(1+b)/2 (P_{i+1} - P_i) + (1-t)(1+c)(1-b)/2 (P_{i+2} - P_{i+1})$

Let constants be $k_1, k_2, k_3, k_4$.
$T_1 = k_1(P_i - P_{i-1}) + k_2(P_{i+1} - P_i) = -k_1 P_{i-1} + (k_1-k_2)P_i + k_2 P_{i+1}$
$T_2 = k_3(P_{i+1} - P_i) + k_4(P_{i+2} - P_{i+1}) = -k_3 P_i + (k_3-k_4)P_{i+1} + k_4 P_{i+2}$

Transform Matrix $M_{H \to KB}$:
Rows are $P_i, P_{i+1}, T_1, T_2$.
$$M_{trans} = \begin{bmatrix} 0 & 1 & 0 & 0 \\ 0 & 0 & 1 & 0 \\ -k_1 & k_1-k_2 & k_2 & 0 \\ 0 & -k_3 & k_3-k_4 & k_4 \end{bmatrix}$$
$M_{KB} = M_{Hermite} \cdot M_{trans}$.
(Specific values depend on the expansion of $k$ terms).
