### Answer 7.1.18

**Given:**
$A\mathbf{u} = \lambda_1 \mathbf{u}$.
$A^T\mathbf{v} = \lambda_2 \mathbf{v}$ (which means $\mathbf{v}^T A = \lambda_2 \mathbf{v}^T$).
Assume $\lambda_1 \neq \lambda_2$.

**Compute $\mathbf{v}^T A \mathbf{u}$ two ways:**
1.  $\mathbf{v}^T (A \mathbf{u}) = \mathbf{v}^T (\lambda_1 \mathbf{u}) = \lambda_1 (\mathbf{v}^T \mathbf{u})$.
2.  $(\mathbf{v}^T A) \mathbf{u} = (\lambda_2 \mathbf{v}^T) \mathbf{u} = \lambda_2 (\mathbf{v}^T \mathbf{u})$.

**Conclusion:**
$\lambda_1 (\mathbf{v}^T \mathbf{u}) = \lambda_2 (\mathbf{v}^T \mathbf{u})$.
$(\lambda_1 - \lambda_2) (\mathbf{v}^T \mathbf{u}) = 0$.
Since $\lambda_1 \neq \lambda_2$, it must be that $\mathbf{v}^T \mathbf{u} = 0$.
Thus $\mathbf{u}$ and $\mathbf{v}$ are orthogonal.