### Answer 2.1.5

**Matrix:**
$$ \left[ \begin{array}{ccc|c} 1 & 0 & -1 & 0 \\ -2 & 3 & -1 & 0 \\ -6 & 6 & 0 & 0 \end{array} \right] $$

**Elimination:**
1.  $R_2 \leftarrow R_2 + 2R_1$: $(-2+2, 3+0, -1-2) \to (0, 3, -3)$.
2.  $R_3 \leftarrow R_3 + 6R_1$: $(-6+6, 6+0, 0-6) \to (0, 6, -6)$.
    $$ \left[ \begin{array}{ccc|c} 1 & 0 & -1 & 0 \\ 0 & 3 & -3 & 0 \\ 0 & 6 & -6 & 0 \end{array} \right] $$
3.  $R_3 \leftarrow R_3 - 2R_2$: $(0, 6-6, -6-(-6)) \to (0, 0, 0)$.
    $$ \left[ \begin{array}{ccc|c} 1 & 0 & -1 & 0 \\ 0 & 3 & -3 & 0 \\ 0 & 0 & 0 & 0 \end{array} \right] $$

**Back Substitution:**
$x_3$ is free ($t$).
$3x_2 - 3t = 0 \implies x_2 = t$.
$x_1 - t = 0 \implies x_1 = t$.

**Solution:**
$$ \mathbf{x} = t(1, 1, 1) $$