### Answer 2.1.8

**Matrix:**
$$ \left[ \begin{array}{cccc|c} 3 & -6 & -1 & 1 & 12 \\ -1 & 2 & 2 & 3 & 1 \\ 6 & -8 & -3 & -2 & 9 \end{array} \right] $$

**Elimination:**
1.  Swap $R_1, R_2$ (and mult new $R_1$ by -1 for pivot 1):
    $$ \left[ \begin{array}{cccc|c} 1 & -2 & -2 & -3 & -1 \\ 3 & -6 & -1 & 1 & 12 \\ 6 & -8 & -3 & -2 & 9 \end{array} \right] $$
2.  $R_2 \leftarrow R_2 - 3R_1$: $(0, 0, 5, 10 \mid 15)$.
3.  $R_3 \leftarrow R_3 - 6R_1$: $(0, 4, 9, 16 \mid 15)$.
    $$ \left[ \begin{array}{cccc|c} 1 & -2 & -2 & -3 & -1 \\ 0 & 0 & 5 & 10 & 15 \\ 0 & 4 & 9 & 16 & 15 \end{array} \right] $$
4.  Swap $R_2, R_3$:
    $$ \left[ \begin{array}{cccc|c} 1 & -2 & -2 & -3 & -1 \\ 0 & 4 & 9 & 16 & 15 \\ 0 & 0 & 5 & 10 & 15 \end{array} \right] $$

**Back Substitution:**
1.  $R_3$: $5x_3 + 10x_4 = 15$. Divide by 5: $x_3 + 2x_4 = 3$.
    $x_4$ is free ($t$). $x_3 = 3 - 2t$.
2.  $R_2$: $4x_2 + 9(3-2t) + 16t = 15$.
    $4x_2 + 27 - 18t + 16t = 15$.
    $4x_2 - 2t = -12 \implies 2x_2 = t - 6 \implies x_2 = -3 + 0.5t$.
3.  $R_1$: $x_1 - 2(-3 + 0.5t) - 2(3 - 2t) - 3t = -1$.
    $x_1 + 6 - t - 6 + 4t - 3t = -1$.
    $x_1 + 0 = -1 \implies x_1 = -1$.

**Solution:**
$$ \mathbf{x} = \begin{bmatrix} -1 \\ -3 \\ 3 \\ 0 \end{bmatrix} + t \begin{bmatrix} 0 \\ 0.5 \\ -2 \\ 1 \end{bmatrix} $$