### Answer 2.1.9

**Matrix:**
$$ \left[ \begin{array}{cccc|c} 1 & 4 & 9 & 2 & 0 \\ 2 & 2 & 6 & -3 & 0 \\ 2 & 7 & 16 & 3 & 0 \end{array} \right] $$

**Elimination:**
1.  $R_2 \leftarrow R_2 - 2R_1$: $(0, -6, -12, -7 \mid 0)$.
2.  $R_3 \leftarrow R_3 - 2R_1$: $(0, -1, -2, -1 \mid 0)$.
    $$ \left[ \begin{array}{cccc|c} 1 & 4 & 9 & 2 & 0 \\ 0 & -6 & -12 & -7 & 0 \\ 0 & -1 & -2 & -1 & 0 \end{array} \right] $$
3.  Swap $R_2, R_3$ (and negate for pivot 1):
    $$ \left[ \begin{array}{cccc|c} 1 & 4 & 9 & 2 & 0 \\ 0 & 1 & 2 & 1 & 0 \\ 0 & -6 & -12 & -7 & 0 \end{array} \right] $$
4.  $R_3 \leftarrow R_3 + 6R_2$:
    $0, -6+6, -12+12, -7+6 \implies (0, 0, 0, -1 \mid 0)$.

**Back Substitution:**
1.  $-x_4 = 0 \implies x_4 = 0$.
2.  $x_2 + 2x_3 + x_4 = 0 \implies x_2 + 2x_3 = 0$.
    $x_3$ is free ($t$). $x_2 = -2t$.
3.  $x_1 + 4(-2t) + 9t + 2(0) = 0$.
    $x_1 - 8t + 9t = 0 \implies x_1 + t = 0 \implies x_1 = -t$.

**Solution:**
$$ \mathbf{x} = t(-1, -2, 1, 0) $$