### Exercise 2.1.14

What is wrong with the following way of "solving" Exercise 2.1.13?

$$
\begin{bmatrix}
3 & -6 & -1 & 1 & 5 \\
-1 & 2 & 2 & 3 & 3 \\
6 & -8 & -3 & -2 & 1
\end{bmatrix}
\xrightarrow{r_1 \leftrightarrow r_2}
\begin{bmatrix}
-1 & 2 & 2 & 3 & 3 \\
3 & -6 & -1 & 1 & 5 \\
6 & -8 & -3 & -2 & 1
\end{bmatrix}
$$

$$
\xrightarrow[r_3 \leftarrow r_3 - 2r_2]{r_1 \leftarrow r_1}
\begin{bmatrix}
-1 & 2 & 2 & 3 & 3 \\
0 & -4 & 1 & 4 & 9 \\
0 & 4 & -1 & -4 & -9
\end{bmatrix}
\xrightarrow{r_3 \leftarrow r_3 + r_2}
\begin{bmatrix}
-1 & 2 & 2 & 3 & 3 \\
0 & -4 & 1 & 4 & 9 \\
0 & 0 & 0 & 0 & 0
\end{bmatrix}
$$

$$
x_3 = s, \quad x_4 = t,
$$

$$
-4x_2 + s + 4t = 9 \implies x_2 = -\frac{9}{4} + \frac{1}{4}s + t,
$$

$$
-x_1 + 2x_2 + 2s + 3t = 3,
$$

$$
x_1 = -3 + 2\left(-\frac{9}{4} + \frac{1}{4}s + t\right) + 2s + 3t = \frac{5}{2}s + 5t - \frac{15}{2}
$$

and so

$$
\mathbf{x} = 
\begin{bmatrix}
-15/2 \\ -9/4 \\ 0 \\ 0
\end{bmatrix}
+
\begin{bmatrix}
5/2 \\ 1/4 \\ 1 \\ 0
\end{bmatrix}s
+
\begin{bmatrix}
5 \\ 1 \\ 0 \\ 1
\end{bmatrix}t.
$$