### Answer 1.1.8

**Relation:** $\mathbf{r}_i = \vec{OO'} + \mathbf{r}_i'$. Let $\mathbf{c} = \vec{OO'}$. So $\mathbf{r}_i = \mathbf{c} + \mathbf{r}_i'$.
The center of mass in system O is $\mathbf{r} = \frac{1}{M} \sum m_i \mathbf{r}_i$.
In the new system, let's calculate the position vector of the same physical point $\mathbf{r}$ relative to $O'$:
$\mathbf{r}'_{cm} = \mathbf{r} - \mathbf{c} = \frac{1}{M} \sum m_i \mathbf{r}_i - \mathbf{c}$.
Substitute $\mathbf{r}_i = \mathbf{c} + \mathbf{r}_i'$:
$\mathbf{r}'_{cm} = \frac{1}{M} \sum m_i (\mathbf{c} + \mathbf{r}_i') - \mathbf{c}$
$= \frac{1}{M} (\sum m_i \mathbf{c} + \sum m_i \mathbf{r}_i') - \mathbf{c}$
Since $\mathbf{c}$ is constant, $\sum m_i \mathbf{c} = \mathbf{c} \sum m_i = \mathbf{c} M$.
$= \frac{1}{M} (M\mathbf{c} + \sum m_i \mathbf{r}_i') - \mathbf{c}$
$= \mathbf{c} + \frac{1}{M} \sum m_i \mathbf{r}_i' - \mathbf{c}$
$= \frac{1}{M} \sum m_i \mathbf{r}_i'$.
This matches the formula definition applied in the new system.