### Answer 1.1.11

**Opposite Edges:** Consider edges $AB$ and $CD$.
Midpoint of $AB$: $\mathbf{m}_{ab} = \frac{1}{2}(\mathbf{a} + \mathbf{b})$.
Midpoint of $CD$: $\mathbf{m}_{cd} = \frac{1}{2}(\mathbf{c} + \mathbf{d})$.
**Midpoint of the Line Joining Edges:**
$\mathbf{M} = \frac{1}{2}(\mathbf{m}_{ab} + \mathbf{m}_{cd})$
$= \frac{1}{2}(\frac{1}{2}(\mathbf{a} + \mathbf{b}) + \frac{1}{2}(\mathbf{c} + \mathbf{d}))$
$= \frac{1}{4}(\mathbf{a} + \mathbf{b} + \mathbf{c} + \mathbf{d})$.
This is exactly the definition of the centroid from Ex 1.1.10.
Since this derivation works for any pair of opposite edges, all such lines meet at $\mathbf{M}$.