### Answer 5.1.11

Let $P = A(A^T A)^{-1} A^T$.

**1. Symmetric ($P^T = P$):**
$P^T = (A(A^T A)^{-1} A^T)^T$.
Using $(ABC)^T = C^T B^T A^T$ and $(M^{-1})^T = (M^T)^{-1}$:
$P^T = (A^T)^T ((A^T A)^{-1})^T A^T$.
$P^T = A ((A^T A)^T)^{-1} A^T$.
Inside inverse: $(A^T A)^T = A^T (A^T)^T = A^T A$. This matrix is symmetric.
$P^T = A (A^T A)^{-1} A^T = P$.
So $P$ is symmetric.

**2. Idempotent ($P^2 = P$):**
$P^2 = P \cdot P = [A(A^T A)^{-1} A^T] [A(A^T A)^{-1} A^T]$.
Associativity: $A(A^T A)^{-1} \underbrace{(A^T A) (A^T A)^{-1}}_{I} A^T$.
$P^2 = A(A^T A)^{-1} I A^T = A(A^T A)^{-1} A^T = P$.
So $P$ is idempotent.