### Answer 5.2.7

**Given:** $\mathbf{q}_1 = \frac{1}{3}(-1, 2, 2)^T$, $\mathbf{q}_2 = \frac{1}{3}(2, -1, 2)^T$.

1.  **Verify Orthonormality:**
    $\|\mathbf{q}_1\|^2 = \frac{1}{9}(1+4+4) = 1$.
    $\|\mathbf{q}_2\|^2 = \frac{1}{9}(4+1+4) = 1$.
    $\mathbf{q}_1 \cdot \mathbf{q}_2 = \frac{1}{9}(-2 - 2 + 4) = 0$.
    They are orthonormal.

2.  **Find $\mathbf{q}_3$:**
    For 3D, $\mathbf{q}_3$ can be the cross product $\mathbf{q}_1 \times \mathbf{q}_2$ (or $-\mathbf{q}_1 \times \mathbf{q}_2$).
    Ignore $1/3$ for calculation, re-scale later.
    $\mathbf{u} = (-1, 2, 2)$, $\mathbf{v} = (2, -1, 2)$.
    $\mathbf{w} = \mathbf{u} \times \mathbf{v} = \begin{vmatrix} \mathbf{i} & \mathbf{j} & \mathbf{k} \\ -1 & 2 & 2 \\ 2 & -1 & 2 \end{vmatrix}$
    $x = (2)(2) - (2)(-1) = 4 + 2 = 6$.
    $y = -((-1)(2) - (2)(2)) = -(-2 - 4) = 6$.
    $z = (-1)(-1) - (2)(2) = 1 - 4 = -3$.
    $\mathbf{w} = (6, 6, -3)$.
    Normalize: $\|\mathbf{w}\| = \sqrt{36+36+9} = \sqrt{81} = 9$.
    $\mathbf{q}_3 = \frac{1}{9}(6, 6, -3) = \frac{1}{3}(2, 2, -1)$.

**Result:** $\mathbf{q}_3 = \frac{1}{3}(2, 2, -1)^T$.