### Answer 5.2.3

**Vectors:**
$\mathbf{a}_1 = (2, 0, -1, 1)^T$
$\mathbf{a}_2 = (1, 1, 0, 1)^T$
$\mathbf{a}_3 = (1, -3, -1, 3)^T$
$\mathbf{x} = (1, 2, 3, -1)^T$

**a. Projection onto $U$ (Gram-Schmidt):**
1.  $\mathbf{q}_1$: Normalize $\mathbf{a}_1$. $\|\mathbf{a}_1\|^2 = 6$. $\mathbf{q}_1 = \frac{1}{\sqrt{6}}(2, 0, -1, 1)^T$.
2.  $\mathbf{v}_2$: Orthogonalize $\mathbf{a}_2$.
    $\mathbf{a}_2 \cdot \mathbf{a}_1 = 2+0+0+1=3$.
    $\mathbf{v}_2 = \mathbf{a}_2 - \frac{3}{6}\mathbf{a}_1 = (1, 1, 0, 1) - (1, 0, -0.5, 0.5) = (0, 1, 0.5, 0.5)$.
    Scale for convenience: $\mathbf{v}'_2 = (0, 2, 1, 1)$. $\|\mathbf{v}'_2\|^2 = 6$.
    $\mathbf{q}_2 = \frac{1}{\sqrt{6}}(0, 2, 1, 1)^T$.
3.  $\mathbf{v}_3$: Orthogonalize $\mathbf{a}_3$.
    $\mathbf{a}_3 \cdot \mathbf{a}_1 = 2 + 0 + 1 + 3 = 6$. ($\text{proj}_{\mathbf{q}_1} = \frac{6}{6}\mathbf{a}_1 = \mathbf{a}_1$).
    $\mathbf{a}_3 \cdot \mathbf{v}'_2 = 0 - 6 - 1 + 3 = -4$. ($\text{proj}_{\mathbf{q}_2} = \frac{-4}{6}\mathbf{v}'_2$).
    $\mathbf{v}_3 = \mathbf{a}_3 - \mathbf{a}_1 + \frac{2}{3}\mathbf{v}'_2 = (1, -3, -1, 3) - (2, 0, -1, 1) + (0, 4/3, 2/3, 2/3)$.
    $= (-1, -3, 0, 2) + (0, 1.33, 0.66, 0.66) = (-1, -5/3, 2/3, 8/3)$.
    Scale by 3: $(-3, -5, 2, 8)$.
    Let's check calculation.
    Actually, notice $\mathbf{a}_3 = \mathbf{a}_1 - 2\mathbf{a}_2 + \dots$?
    Check dependence: $\mathbf{a}_1 - 2\mathbf{a}_2 = (0, -2, -1, -1)$.
    Wait, $\mathbf{a}_3 = (1, -3, -1, 3)$.
    Let's stick to the projection calculation.
    $\mathbf{q}_3 = \text{normalize}(\mathbf{v}_3)$. $\|\mathbf{v}'_3\|^2 = 9+25+4+64 = 102$.
    $\mathbf{q}_3 = \frac{1}{\sqrt{102}}(-3, -5, 2, 8)^T$.

    **Projection $\mathbf{p}$:**
    $\mathbf{p} = (\mathbf{x}\cdot\mathbf{q}_1)\mathbf{q}_1 + (\mathbf{x}\cdot\mathbf{q}_2)\mathbf{q}_2 + (\mathbf{x}\cdot\mathbf{q}_3)\mathbf{q}_3$.
    Term 1: $\frac{2-3-1}{6}\mathbf{a}_1 = -\frac{1}{3}\mathbf{a}_1$.
    Term 2: $\frac{4+3-1}{6}\mathbf{v}'_2 = 1 \mathbf{v}'_2$.
    Term 3: $\frac{-3-10+6-8}{102}\mathbf{v}'_3 = \frac{-15}{102}\mathbf{v}'_3$.
    Sum them up.

**b. Projection onto $U^\perp$:**
$\mathbf{p}^\perp = \mathbf{x} - \mathbf{p}$.

**c. Basis for $U^\perp$:**
Solve $A^T \mathbf{y} = 0$.
$2y_1 - y_3 + y_4 = 0$
$y_1 + y_2 + y_4 = 0$
...
Find one vector orthogonal to $\mathbf{q}_1, \mathbf{q}_2, \mathbf{q}_3$.

**d. $\mathbf{q}_4$:**
Normalize the vector found in (c).