### Answer 16.2

The third-order Taylor series requires the second derivative of the function $f(x, y(x))$ with respect to $x$.
Given $y' = f(x, y)$.

**1. First Total Derivative ($y''$):**
$$y'' = f'(x, y) = \frac{d}{dx}f(x, y) = \frac{\partial f}{\partial x} + \frac{\partial f}{\partial y}\frac{dy}{dx}$$
$$y'' = f_x + f_y f$$

**2. Second Total Derivative ($y'''$):**
We differentiate $y''$ with respect to $x$:
$$y''' = \frac{d}{dx}(f_x + f_y f)$$
$$y''' = \frac{d}{dx}(f_x) + \frac{d}{dx}(f_y f)$$

Apply chain rule to terms:
$$\frac{d}{dx}(f_x) = f_{xx} + f_{xy} y' = f_{xx} + f_{xy} f$$
$$\frac{d}{dx}(f_y f) = (\frac{d}{dx}f_y) f + f_y (\frac{d}{dx}f)$$
$$= (f_{yx} + f_{yy} y') f + f_y (f_x + f_y y')$$
$$= (f_{yx} + f_{yy} f) f + f_y (f_x + f_y f)$$

**3. Combine and Simplify:**
Assuming continuity ($f_{xy} = f_{yx}$):
$$y''' = (f_{xx} + f_{xy} f) + (f_{xy} f + f_{yy} f^2) + (f_y f_x + f_y^2 f)$$
$$y''' = f_{xx} + 2f_{xy} f + f_{yy} f^2 + f_x f_y + f_y^2 f$$
