### Answer 16.3

**1. Heun's Method Formula**
$$y_{i+1} = y_i + \frac{h}{2} [f(t_i, y_i) + f(t_i + h, y_i + h f(t_i, y_i))]$$

**2. Differential Equation**
$$y'(t) = v_0 - gt$$
Here, $f(t, y) = v_0 - gt$. Note that $f$ is independent of $y$.

**3. Apply Method**
$$f(t_i) = v_0 - gt_i$$
$$f(t_i + h) = v_0 - g(t_i + h) = v_0 - gt_i - gh$$

Substitute into Heun's formula:
$$y_{i+1} = y_i + \frac{h}{2} [ (v_0 - gt_i) + (v_0 - gt_i - gh) ]$$
$$y_{i+1} = y_i + \frac{h}{2} [ 2v_0 - 2gt_i - gh ]$$
$$y_{i+1} = y_i + v_0 h - gt_i h - \frac{1}{2}gh^2$$

**4. Verification with Exact Solution**
Exact solution integration: $\int_{t}^{t+h} (v_0 - g\tau) d\tau$.
$$y(t+h) - y(t) = [v_0 \tau - \frac{1}{2}g\tau^2]_t^{t+h}$$
$$= v_0(t+h) - \frac{1}{2}g(t+h)^2 - (v_0 t - \frac{1}{2}gt^2)$$
$$= v_0 h - \frac{1}{2}g(t^2 + 2th + h^2) + \frac{1}{2}gt^2$$
$$= v_0 h - \frac{1}{2}gt^2 - gth - \frac{1}{2}gh^2 + \frac{1}{2}gt^2$$
$$= v_0 h - gth - \frac{1}{2}gh^2$$

The expressions match exactly.
