### Answer 6.3.4

**Proof of Statement 11:**
Let $\mathbf{u}=(u_1, u_2, u_3)$, $\mathbf{v}=(v_1, v_2, v_3)$, $\mathbf{w}=(w_1, w_2, w_3)$.
Calculate $\mathbf{u} \cdot (\mathbf{v} \times \mathbf{w})$.
$\mathbf{v} \times \mathbf{w} = (v_2 w_3 - v_3 w_2, v_3 w_1 - v_1 w_3, v_1 w_2 - v_2 w_1)$.
Dot product:
$u_1(v_2 w_3 - v_3 w_2) + u_2(v_3 w_1 - v_1 w_3) + u_3(v_1 w_2 - v_2 w_1)$.
This is exactly the expansion of the determinant $det(\mathbf{u}, \mathbf{v}, \mathbf{w})$ along the first row.
Since determinant is unchanged by cyclic permutation of rows ($\mathbf{u}, \mathbf{v}, \mathbf{w} \to \mathbf{v}, \mathbf{w}, \mathbf{u}$ involves 2 swaps), the equality holds.