### Answer 6.3.7

**Lagrange's Identity:**
$(\mathbf{a} \times \mathbf{b}) \cdot (\mathbf{c} \times \mathbf{d})$.
This is a scalar triple product of vectors $\mathbf{a} \times \mathbf{b}$, $\mathbf{c}$, and $\mathbf{d}$? No.
Let $\mathbf{u} = \mathbf{a} \times \mathbf{b}$.
$\mathbf{u} \cdot (\mathbf{c} \times \mathbf{d}) = \mathbf{d} \cdot (\mathbf{u} \times \mathbf{c})$ (Cyclic permutation of scalar triple product).
$= \mathbf{d} \cdot ((\mathbf{a} \times \mathbf{b}) \times \mathbf{c})$.
Use vector triple product rule (Statement 12): $(\mathbf{a} \times \mathbf{b}) \times \mathbf{c} = (\mathbf{a} \cdot \mathbf{c})\mathbf{b} - (\mathbf{b} \cdot \mathbf{c})\mathbf{a}$.
Note order: $(\mathbf{A} \times \mathbf{B}) \times \mathbf{C} = - \mathbf{C} \times (\mathbf{A} \times \mathbf{B}) = - [(\mathbf{C} \cdot \mathbf{B})\mathbf{A} - (\mathbf{C} \cdot \mathbf{A})\mathbf{B}] = (\mathbf{C} \cdot \mathbf{A})\mathbf{B} - (\mathbf{C} \cdot \mathbf{B})\mathbf{A}$.
So substitute back:
$= \mathbf{d} \cdot [ (\mathbf{a} \cdot \mathbf{c})\mathbf{b} - (\mathbf{b} \cdot \mathbf{c})\mathbf{a} ]$.
Distribute dot product:
$= (\mathbf{a} \cdot \mathbf{c})(\mathbf{b} \cdot \mathbf{d}) - (\mathbf{b} \cdot \mathbf{c})(\mathbf{a} \cdot \mathbf{d})$.
This matches the formula.