### Answer 6.3.3

**Vectors:** $\mathbf{u}=(1,-1,0)$, $\mathbf{v}=(1,2,0)$, $\mathbf{w}=(1,0,3)$.

**Statement 11 (Scalar Triple Product):**
$\mathbf{v} \times \mathbf{w} = (6, -3, -2)$.
$\mathbf{u} \cdot (\mathbf{v} \times \mathbf{w}) = 1(6) - 1(-3) + 0(-2) = 9$.
Determinant: $\begin{vmatrix} 1 & -1 & 0 \\ 1 & 2 & 0 \\ 1 & 0 & 3 \end{vmatrix}$. Expand col 3: $3(2 - (-1)) = 9$. Verified.

**Statement 12 (Vector Triple Product):**
$(\mathbf{u} \times \mathbf{v}) \times \mathbf{w}$.
$\mathbf{u} \times \mathbf{v} = (0, 0, 3)$ (from Ex 6.3.1).
$(0, 0, 3) \times (1, 0, 3) = (0, 3, 0)$.
RHS: $(\mathbf{u} \cdot \mathbf{w})\mathbf{v} - (\mathbf{v} \cdot \mathbf{w})\mathbf{u}$.
$\mathbf{u} \cdot \mathbf{w} = 1$. $\mathbf{v} \cdot \mathbf{w} = 1$.
$1(1,2,0) - 1(1,-1,0) = (0, 3, 0)$. Verified.

**Statement 13 (Jacobi-like):**
$\mathbf{u} \times (\mathbf{v} \times \mathbf{w}) = (1,-1,0) \times (6,-3,-2) = (2, 2, 3)$.
RHS: $(\mathbf{u} \cdot \mathbf{w})\mathbf{v} - (\mathbf{u} \cdot \mathbf{v})\mathbf{w}$.
$\mathbf{u} \cdot \mathbf{w} = 1$. $\mathbf{u} \cdot \mathbf{v} = -1$.
$1(1,2,0) - (-1)(1,0,3) = (1,2,0) + (1,0,3) = (2, 2, 3)$. Verified.