### Answer 2.3.4

**Matrix:**
$$ \left[ \begin{array}{cccc|c} 3 & -6 & -1 & 1 & 12 \\ -1 & 2 & 2 & 3 & 1 \\ 6 & -8 & -3 & -2 & 9 \end{array} \right] $$

**Gauss-Jordan Elimination:**
1.  Swap $R_1, R_2$ and negate $R_1$:
    $$ \left[ \begin{array}{cccc|c} 1 & -2 & -2 & -3 & -1 \\ 3 & -6 & -1 & 1 & 12 \\ 6 & -8 & -3 & -2 & 9 \end{array} \right] $$
2.  Eliminate Col 1:
    $R_2 \leftarrow R_2 - 3R_1 \implies (0, 0, 5, 10 \mid 15)$.
    $R_3 \leftarrow R_3 - 6R_1 \implies (0, 4, 9, 16 \mid 15)$.
3.  Swap $R_2, R_3$ to put pivot ($x_2$) in place:
    $$ \left[ \begin{array}{cccc|c} 1 & -2 & -2 & -3 & -1 \\ 0 & 4 & 9 & 16 & 15 \\ 0 & 0 & 5 & 10 & 15 \end{array} \right] $$
4.  Scale pivots to 1:
    $R_2 \leftarrow R_2/4 \implies (0, 1, 2.25, 4 \mid 3.75)$.
    $R_3 \leftarrow R_3/5 \implies (0, 0, 1, 2 \mid 3)$.
5.  Eliminate upwards (Col 3, $x_3$):
    $R_2 \leftarrow R_2 - 2.25R_3 \implies R_2: (0, 1, 0, 4 - 2.25(2) \mid 3.75 - 2.25(3)) = (0, 1, 0, -0.5 \mid -3)$.
    $R_1 \leftarrow R_1 + 2R_3 \implies R_1: (1, -2, 0, 1 \mid 5)$.
6.  Eliminate upwards (Col 2, $x_2$):
    $R_1 \leftarrow R_1 + 2R_2 \implies R_1: (1, 0, 0, 1 + 2(-0.5) \mid 5 + 2(-3)) = (1, 0, 0, 0 \mid -1)$.

**RREF:**
$$ \left[ \begin{array}{cccc|c} 1 & 0 & 0 & 0 & -1 \\ 0 & 1 & 0 & -0.5 & -3 \\ 0 & 0 & 1 & 2 & 3 \end{array} \right] $$

**Solution:**
$x_1 = -1$.
$x_2 = -3 + 0.5t$.
$x_3 = 3 - 2t$.
$x_4 = t$.
$$ \mathbf{x} = (-1, -3, 3, 0) + t(0, 0.5, -2, 1) $$