### Answer 2.3.3

**Matrix:**
$$ \left[ \begin{array}{ccc|c} 1 & 0 & -1 & 0 \\ -2 & 3 & -1 & 0 \\ -6 & 6 & 0 & 0 \end{array} \right] $$

**Gauss-Jordan Elimination:**
1.  Eliminate Col 1:
    $R_2 \leftarrow R_2 + 2R_1 \implies (0, 3, -3)$.
    $R_3 \leftarrow R_3 + 6R_1 \implies (0, 6, -6)$.
2.  Scale $R_2$ to make pivot 1:
    $R_2 \leftarrow \frac{1}{3}R_2 \implies (0, 1, -1)$.
    $$ \left[ \begin{array}{ccc|c} 1 & 0 & -1 & 0 \\ 0 & 1 & -1 & 0 \\ 0 & 6 & -6 & 0 \end{array} \right] $$
3.  Eliminate Col 2 ($x_2$) from $R_3$:
    $R_3 \leftarrow R_3 - 6R_2 \implies (0, 0, 0)$.
4.  Eliminate Col 2 from $R_1$:
    Already 0.

**RREF:**
$$ \left[ \begin{array}{ccc|c} 1 & 0 & -1 & 0 \\ 0 & 1 & -1 & 0 \\ 0 & 0 & 0 & 0 \end{array} \right] $$

**Solution:**
$x_1 - x_3 = 0 \implies x_1 = t$.
$x_2 - x_3 = 0 \implies x_2 = t$.
$x_3 = t$ (Free).
$$ \mathbf{x} = t(1, 1, 1) $$