### Answer 4.1.16

**Equation 4.27:** $\mathbf{y}_B = T_{A,B} \mathbf{x}_A$.
**Example 4.1.12:**
$T = \text{projection onto } x \text{ axis}$.
Basis $A = \{(1,1), (-1,1)\}$. Basis $B = \{(1,0), (0,1)\}$.
$T(1,1) = (1,0) = 1\mathbf{b}_1 + 0\mathbf{b}_2$.
$T(-1,1) = (-1,0) = -1\mathbf{b}_1 + 0\mathbf{b}_2$.
Matrix $T_{A,B} = \begin{bmatrix} 1 & -1 \\ 0 & 0 \end{bmatrix}$.
Check vector $\mathbf{x} = (0,2) = 1(1,1) + 1(-1,1) \implies \mathbf{x}_A = (1,1)^T$.
$T(\mathbf{x}) = (0,0)$.
$T_{A,B} \mathbf{x}_A = \begin{bmatrix} 1 & -1 \\ 0 & 0 \end{bmatrix} \begin{bmatrix} 1 \\ 1 \end{bmatrix} = \begin{bmatrix} 0 \\ 0 \end{bmatrix}$.
Matches $\mathbf{y}_B = (0,0)^T$. Verified.