### Answer 4.1.1

**a. Proof of Lemma 4.1.1:**
Lemma: $T(c\mathbf{x} + d\mathbf{y}) = cT(\mathbf{x}) + dT(\mathbf{y})$.
Proof:
$T(c\mathbf{x} + d\mathbf{y}) = T(c\mathbf{x}) + T(d\mathbf{y})$ (by Additivity Axiom)
$= cT(\mathbf{x}) + dT(\mathbf{y})$ (by Homogeneity Axiom).

**Proof of Corollary 4.1.1:**
Generalize to $n$ vectors by induction.
$T(\sum c_i \mathbf{x}_i) = \sum c_i T(\mathbf{x}_i)$.

**b. Proof $T(\mathbf{0}) = \mathbf{0}$:**
$T(\mathbf{0}) = T(0 \cdot \mathbf{x}) = 0 \cdot T(\mathbf{x}) = \mathbf{0}$.
(Using homogeneity with scalar 0).