### Answer 3.4.9

**Proof:**
We show $Null(B) \subseteq Null(AB)$ and $Null(AB) \subseteq Null(B)$.

1.  Let $\mathbf{x} \in Null(B)$. Then $B\mathbf{x} = \mathbf{0}$.
    Multiply by $A$: $AB\mathbf{x} = A(\mathbf{0}) = \mathbf{0}$.
    So $\mathbf{x} \in Null(AB)$.

2.  Let $\mathbf{x} \in Null(AB)$. Then $AB\mathbf{x} = \mathbf{0}$.
    Since $A$ is **invertible**, multiply by $A^{-1}$:
    $A^{-1}(AB\mathbf{x}) = A^{-1}\mathbf{0}$.
    $(A^{-1}A)B\mathbf{x} = \mathbf{0}$.
    $I B \mathbf{x} = \mathbf{0} \implies B\mathbf{x} = \mathbf{0}$.
    So $\mathbf{x} \in Null(B)$.

Since subsets go both ways, the sets are equal.