### Answer 2.5.4

**Matrix:**
$$ \begin{bmatrix} 0 & -6 & 2 \\ 3 & -1 & 0 \\ 4 & 3 & -2 \end{bmatrix} $$

**Reduction:**
1.  Swap $R_1, R_2$:
    $$ \begin{bmatrix} 3 & -1 & 0 & 0 & 1 & 0 \\ 0 & -6 & 2 & 1 & 0 & 0 \\ 4 & 3 & -2 & 0 & 0 & 1 \end{bmatrix} $$
2.  Eliminate $R_3$ ($R_3 \leftarrow 3R_3 - 4R_1$):
    $3(4, 3, -2) - 4(3, -1, 0) = (12-12, 9+4, -6-0) = (0, 13, -6)$.
    RHS: $3(0,0,1) - 4(0,1,0) = (0, -4, 3)$.
3.  Eliminate $R_3$ using $R_2$:
    $R_3 \leftarrow 6R_3 + 13R_2$:
    $6(0, 13, -6) + 13(0, -6, 2) = (0, 78-78, -36+26) = (0, 0, -10)$.
    RHS: $6(0, -4, 3) + 13(1, 0, 0) = (0, -24, 18) + (13, 0, 0) = (13, -24, 18)$.
4.  Normalize $R_3$: $(0, 0, 1 \mid -1.3, 2.4, -1.8)$.
5.  Back-substitute.

**Result:**
$$ A^{-1} = \begin{bmatrix} 0.2 & -0.6 & 0.2 \\ 0.6 & -0.8 & 0.6 \\ 1.3 & -2.4 & 1.8 \end{bmatrix} = \frac{1}{10} \begin{bmatrix} 2 & -6 & 2 \\ 6 & -8 & 6 \\ 13 & -24 & 18 \end{bmatrix} $$