### Answer 4.1.8

**Conditions:**
1. $T(1,1) = (1,1,1)^T$
2. $T(1,-1) = (1,-1,-1)^T$

**Find Basis Images:**
$\mathbf{e}_1 = \frac{1}{2} ((1,1) + (1,-1))$.
$T(\mathbf{e}_1) = \frac{1}{2} (T(1,1) + T(1,-1)) = \frac{1}{2} ( (1,1,1) + (1,-1,-1) ) = \frac{1}{2} (2, 0, 0) = (1, 0, 0)^T$.
$\mathbf{e}_2 = \frac{1}{2} ((1,1) - (1,-1))$.
$T(\mathbf{e}_2) = \frac{1}{2} ( (1,1,1) - (1,-1,-1) ) = \frac{1}{2} (0, 2, 2) = (0, 1, 1)^T$.

**Matrix:**
$$ [T] = \begin{bmatrix} 1 & 0 \\ 0 & 1 \\ 0 & 1 \end{bmatrix} $$