### Answer 4.1.11

**Process:**
1.  Rotate $-45^\circ$ to align $y=x$ with x-axis.
2.  Stretch x-axis by 2.
3.  Rotate $+45^\circ$ back.

**Matrices:**
$R_{45} = \frac{1}{\sqrt{2}} \begin{bmatrix} 1 & -1 \\ 1 & 1 \end{bmatrix}$.
$S = \begin{bmatrix} 2 & 0 \\ 0 & 1 \end{bmatrix}$ (Stretch along new x, i.e., old $y=x$).
Wait, usually we align $y=x$ to x-axis, stretch x, rotate back.
Rotation $-45$: $R_{-45} = \frac{1}{\sqrt{2}} \begin{bmatrix} 1 & 1 \\ -1 & 1 \end{bmatrix}$.
$T = R_{45} S R_{-45}$.
$T = \frac{1}{2} \begin{bmatrix} 1 & -1 \\ 1 & 1 \end{bmatrix} \begin{bmatrix} 2 & 0 \\ 0 & 1 \end{bmatrix} \begin{bmatrix} 1 & 1 \\ -1 & 1 \end{bmatrix}$
$= \frac{1}{2} \begin{bmatrix} 2 & -1 \\ 2 & 1 \end{bmatrix} \begin{bmatrix} 1 & 1 \\ -1 & 1 \end{bmatrix}$
$= \frac{1}{2} \begin{bmatrix} 3 & 1 \\ 1 & 3 \end{bmatrix} = \begin{bmatrix} 1.5 & 0.5 \\ 0.5 & 1.5 \end{bmatrix}$.