### Answer 4.1.18

**Basis:** $v_k = \sum_{i=0}^k x^i$.
$D(v_k) = \sum_{i=1}^k i x^{i-1}$.
Example $n=2$: Basis $\{1, 1+x, 1+x+x^2\}$.
$D(1) = 0$.
$D(1+x) = 1 = v_0$.
$D(1+x+x^2) = 1+2x = 2(1+x) - 1 = 2v_1 - v_0$.
$D(v_3) = 1+2x+3x^2 = 3(1+x+x^2) - (1+x) - 1 = 3v_2 - v_1 - v_0$? No.
$3(1+x+x^2) = 3+3x+3x^2$. Target $1+2x+3x^2$.
Diff = $-2-x = -(1+x) - 1 = -v_1 - v_0$.
So $D(v_3) = 3v_2 - v_1 - v_0$.
**Pattern:** Column $j$ (for $v_j$) has entries $-1, -1, \dots, -1, j$ (at pos $j$), then 0.
Matrix is upper Hessenberg.