### Answer 4.1.9

**Conditions:**
1. $T(1,1,1) = (1,1)^T$
2. $T(1,-1,-1) = (1,-1)^T$
3. $T(1,1,0) = (1,0)^T$

**Solve for Basis Images:**
Let vectors be $\mathbf{v}_1, \mathbf{v}_2, \mathbf{v}_3$.
$\mathbf{v}_1 + \mathbf{v}_2 = (2, 0, 0) \implies \mathbf{e}_1 = (1, 0, 0)$? No, check vectors.
$\mathbf{v}_1 = (1,1,1), \mathbf{v}_2 = (1,-1,-1)$.
Sum = $(2, 0, 0)$. So $2\mathbf{e}_1 = \mathbf{v}_1 + \mathbf{v}_2$.
$T(\mathbf{e}_1) = 0.5 ( (1,1) + (1,-1) ) = (1, 0)^T$.
From $\mathbf{v}_3 = (1,1,0) = \mathbf{e}_1 + \mathbf{e}_2$.
$\mathbf{e}_2 = \mathbf{v}_3 - \mathbf{e}_1 = (1,1,0) - (1,0,0) = (0,1,0)$.
$T(\mathbf{e}_2) = T(\mathbf{v}_3) - T(\mathbf{e}_1) = (1,0) - (1,0) = (0, 0)^T$.
From $\mathbf{v}_1 = (1,1,1) = \mathbf{e}_1 + \mathbf{e}_2 + \mathbf{e}_3$.
$\mathbf{e}_3 = \mathbf{v}_1 - \mathbf{e}_1 - \mathbf{e}_2$.
$T(\mathbf{e}_3) = (1,1) - (1,0) - (0,0) = (0, 1)^T$.

**Matrix:**
$$ [T] = \begin{bmatrix} 1 & 0 & 0 \\ 0 & 0 & 1 \end{bmatrix} $$