### Answer 3.1.13

**Cancellation Rule Proof:**
Given: $\mathbf{p} + \mathbf{q} = \mathbf{p} + \mathbf{r}$.
By the Axiom of Inverses, there exists a vector $-\mathbf{p}$.
Add $-\mathbf{p}$ to the left side of both expressions:
$-\mathbf{p} + (\mathbf{p} + \mathbf{q}) = -\mathbf{p} + (\mathbf{p} + \mathbf{r})$.
Use Associativity:
$(-\mathbf{p} + \mathbf{p}) + \mathbf{q} = (-\mathbf{p} + \mathbf{p}) + \mathbf{r}$.
Use Inverse property:
$\mathbf{0} + \mathbf{q} = \mathbf{0} + \mathbf{r}$.
Use Identity property:
$\mathbf{q} = \mathbf{r}$.