### Answer 3.1.11

**6. Prove $(-c)\mathbf{p} = -(c\mathbf{p})$:**
$(-c)\mathbf{p} + c\mathbf{p} = (-c + c)\mathbf{p}$ (Distributive law)
$= 0\mathbf{p} = \mathbf{0}$.
Since adding $(-c)\mathbf{p}$ to $c\mathbf{p}$ gives $\mathbf{0}$, $(-c)\mathbf{p}$ is the additive inverse of $c\mathbf{p}$.

**7. Prove $c(\mathbf{p} - \mathbf{q}) = c\mathbf{p} - c\mathbf{q}$:**
$c(\mathbf{p} + (-\mathbf{q})) = c\mathbf{p} + c(-\mathbf{q})$ (Distributive)
Using part 6 (with $c=1$), $c(-\mathbf{q}) = c((-1)\mathbf{q}) = (c(-1))\mathbf{q} = -c\mathbf{q}$.
So $c\mathbf{p} - c\mathbf{q}$.

**8. Prove $(c - d)\mathbf{p} = c\mathbf{p} - d\mathbf{p}$:**
$(c + (-d))\mathbf{p} = c\mathbf{p} + (-d)\mathbf{p}$ (Distributive)
$= c\mathbf{p} + -(d\mathbf{p})$ (By part 6)
$= c\mathbf{p} - d\mathbf{p}$.