### Answer 3.5.13

**Proof:**
$U^\perp = \{ \mathbf{x} \in X \mid \langle \mathbf{x}, \mathbf{u} \rangle = 0, \forall \mathbf{u} \in U \}$.
1.  $\mathbf{0} \in U^\perp$ since $\langle \mathbf{0}, \mathbf{u} \rangle = 0$.
2.  If $\mathbf{x}, \mathbf{y} \in U^\perp$, then $\langle \mathbf{x}+\mathbf{y}, \mathbf{u} \rangle = \langle \mathbf{x}, \mathbf{u} \rangle + \langle \mathbf{y}, \mathbf{u} \rangle = 0+0=0$.
3.  If $\mathbf{x} \in U^\perp$, $\langle c\mathbf{x}, \mathbf{u} \rangle = c\langle \mathbf{x}, \mathbf{u} \rangle = 0$.
Thus $U^\perp$ is a subspace.