### Answer 6.1.14



**Determinant:**
$$ V = \begin{vmatrix} 1 & 1 & 1 \\ a & b & c \\ a^2 & b^2 & c^2 \end{vmatrix} $$
**Row Operations:**
1.  $R_2 \leftarrow R_2 - aR_1 \implies (0, b-a, c-a)$.
2.  $R_3 \leftarrow R_3 - a^2R_1 \implies (0, b^2-a^2, c^2-a^2)$.
    $$ V = \begin{vmatrix} 1 & 1 & 1 \\ 0 & b-a & c-a \\ 0 & b^2-a^2 & c^2-a^2 \end{vmatrix} $$
3.  Factor $(b-a)$ from Col 2 (of submatrix) and $(c-a)$ from Col 3:
    Note: $b^2-a^2 = (b-a)(b+a)$.
    $$ V = (b-a)(c-a) \begin{vmatrix} 1 & 1 & 1 \\ 0 & 1 & 1 \\ 0 & b+a & c+a \end{vmatrix} $$
    Wait, cofactor expansion along Col 1 reduces to $2 \times 2$:
    $$ V = \begin{vmatrix} b-a & c-a \\ (b-a)(b+a) & (c-a)(c+a) \end{vmatrix} = (b-a)(c-a) \begin{vmatrix} 1 & 1 \\ b+a & c+a \end{vmatrix} $$
4.  Solve $2 \times 2$: $(c+a) - (b+a) = c - b$.
    $$ V = (b-a)(c-a)(c-b) $$
    $$ V = (b-a)(c-b)(c-a) $$