### Answer 2.4.18

**Proof (Distributive Law):**
Let $A$ be $m \times n$, and $B, C$ be $n \times p$.
We compare the $(i,j)$ entry of $LHS$ and $RHS$.

**LHS:** $(A(B+C))_{ij} = \sum_{k=1}^n A_{ik} (B+C)_{kj}$.
Since matrix addition is entry-wise: $(B+C)_{kj} = B_{kj} + C_{kj}$.
Substitute: $\sum_{k=1}^n A_{ik} (B_{kj} + C_{kj})$.
Distribute scalar: $\sum_{k=1}^n (A_{ik} B_{kj} + A_{ik} C_{kj})$.
Split sum: $\sum_{k=1}^n A_{ik} B_{kj} + \sum_{k=1}^n A_{ik} C_{kj}$.

**RHS:** $(AB + AC)_{ij} = (AB)_{ij} + (AC)_{ij}$.
By definition of product: $(AB)_{ij} = \sum_{k=1}^n A_{ik} B_{kj}$ and $(AC)_{ij} = \sum_{k=1}^n A_{ik} C_{kj}$.
Sum: $\sum_{k=1}^n A_{ik} B_{kj} + \sum_{k=1}^n A_{ik} C_{kj}$.

Since the entries are identical for all $i,j$, $A(B+C) = AB + AC$.