### Answer 2.4.12

We need $AB = AC$ with $A \neq O$ and $B \neq C$.

**Example:**
Let $A = \begin{bmatrix} 0 & 1 \\ 0 & 0 \end{bmatrix}$.
Let $B = \begin{bmatrix} 1 & 0 \\ 0 & 0 \end{bmatrix}$.
Let $C = \begin{bmatrix} 0 & 0 \\ 0 & 1 \end{bmatrix}$.

**Check $B \neq C$:** True.

**Check Products:**
$AB = \begin{bmatrix} 0 & 1 \\ 0 & 0 \end{bmatrix} \begin{bmatrix} 1 & 0 \\ 0 & 0 \end{bmatrix} = \begin{bmatrix} 0 & 0 \\ 0 & 0 \end{bmatrix}$.
$AC = \begin{bmatrix} 0 & 1 \\ 0 & 0 \end{bmatrix} \begin{bmatrix} 0 & 0 \\ 0 & 1 \end{bmatrix} = \begin{bmatrix} 0 & 1 \\ 0 & 0 \end{bmatrix}$.
Wait, those aren't equal. Let's try matrices that project to zero.

**Better Example:**
Let $A = \begin{bmatrix} 1 & 0 \\ 0 & 0 \end{bmatrix}$.
Let $B = \begin{bmatrix} 0 & 0 \\ 0 & 1 \end{bmatrix}$.
Let $C = \begin{bmatrix} 0 & 0 \\ 0 & 0 \end{bmatrix}$.
$AB = O$, $AC = O$. So $AB=AC$. But $B \neq C$.

**Another Example (Nonzero product):**
$A = \begin{bmatrix} 1 & 0 \\ 0 & 0 \end{bmatrix}$.
$B = \begin{bmatrix} 1 & 1 \\ 0 & 0 \end{bmatrix}$.
$C = \begin{bmatrix} 1 & 0 \\ 0 & 0 \end{bmatrix}$.
$AB = \begin{bmatrix} 1 & 1 \\ 0 & 0 \end{bmatrix}$.
$AC = \begin{bmatrix} 1 & 0 \\ 0 & 0 \end{bmatrix}$. Not equal.

**Correct Example:**
Let $A = \begin{bmatrix} 0 & 1 \\ 0 & 0 \end{bmatrix}$.
Let $B = \begin{bmatrix} 0 & 2 \\ 0 & 0 \end{bmatrix}$.
Let $C = \begin{bmatrix} 0 & 3 \\ 0 & 0 \end{bmatrix}$.
$AB = O$, $AC = O$.

Let's use the property of projection.
$A = \begin{bmatrix} 1 & 0 \\ 0 & 0 \end{bmatrix}$.
$B = \begin{bmatrix} 0 & 0 \\ 0 & 1 \end{bmatrix}$.
$C = \begin{bmatrix} 0 & 0 \\ 0 & 2 \end{bmatrix}$.
$AB = O$. $AC = O$.
Thus $AB = AC$, but $B \neq C$.