### Answer 2.4.1

Given $A = \begin{bmatrix} 2 & 3 \\ 1 & -2 \end{bmatrix}$ and $B = \begin{bmatrix} 3 & -4 \\ 2 & 2 \end{bmatrix}$.

**a. $C = 2A + 3B$**
$2A = \begin{bmatrix} 4 & 6 \\ 2 & -4 \end{bmatrix}$
$3B = \begin{bmatrix} 9 & -12 \\ 6 & 6 \end{bmatrix}$
$C = \begin{bmatrix} 4+9 & 6-12 \\ 2+6 & -4+6 \end{bmatrix} = \begin{bmatrix} 13 & -6 \\ 8 & 2 \end{bmatrix}$

**b. $D = 4A - 3B$**
$4A = \begin{bmatrix} 8 & 12 \\ 4 & -8 \end{bmatrix}$
$3B = \begin{bmatrix} 9 & -12 \\ 6 & 6 \end{bmatrix}$
$D = \begin{bmatrix} 8-9 & 12-(-12) \\ 4-6 & -8-6 \end{bmatrix} = \begin{bmatrix} -1 & 24 \\ -2 & -14 \end{bmatrix}$