- **Recurrence:** $b_{i,k}(t) = \frac{t-t_i}{t_{i+k-1}-t_i} b_{i,k-1}(t) + \frac{t_{i+k}-t}{t_{i+k}-t_{i+1}} b_{i+1,k-1}(t)$.

- **Target:** $k=2$ (Degree 1, Linear), Uniform knots $t_i = i$.

- **Base Case ($k=1$):** $b_{i,1}(t) = 1$ if $t \in [i, i+1)$, else 0.

- **Substitution ($k=2$):**

  $$
  b_{i,2}(t) = \frac{t-i}{(i+1)-i} b_{i,1}(t) + \frac{(i+2)-t}{(i+2)-(i+1)} b_{i+1,1}(t)
  $$

  $$
  b_{i,2}(t) = (t-i) b_{i,1}(t) + (2 - (t-i)) b_{i+1,1}(t)
  $$

- **Result:** This defines the "hat function":

  - $t - i$ (linear ramp up) for $t \in [i, i+1]$.

  - $2 - (t-i)$ (linear ramp down) for $t \in [i+1, i+2]$.

  - 0 otherwise. This matches Equation 15.16.
