### Answer 13.1

Equation: $x''(t) - 6x'(t) + 9x(t) = 9t + 3$.

**1. Homogeneous Solution $g(t)$**
Auxiliary equation: $r^2 - 6r + 9 = 0$.
$(r-3)^2 = 0 \implies r = 3$ (repeated root).
$$g(t) = Ae^{3t} + Bte^{3t}$$

**2. Particular Solution $p(t)$**
Assume $p(t) = Ct + D$ (since RHS is linear).
$p'(t) = C$, $p''(t) = 0$.
Substitute into ODE:
$0 - 6(C) + 9(Ct + D) = 9t + 3$
$9Ct + (9D - 6C) = 9t + 3$

Equate coefficients:
$9C = 9 \implies C = 1$
$9D - 6(1) = 3 \implies 9D = 9 \implies D = 1$
$$p(t) = t + 1$$

**3. General Solution**
$$x(t) = Ae^{3t} + Bte^{3t} + t + 1$$
