### Answer 13.6

**1. Position Function**
From Equation (13.96), with $x_0=50$, $v_0=0$ (dropped from rest), $g=9.8$, $k=1$.
$x(t) = 50 + \frac{9.8}{1}t + \frac{1(0) - 9.8}{1^2}(1 - e^{-1t})$
$f(t) = 50 + 9.8t - 9.8(1 - e^{-t}) = 0$ (Ground level).
$f(t) = 50 + 9.8t - 9.8 + 9.8e^{-t} = 40.2 + 9.8t + 9.8e^{-t}$.
We want to find root of $f(t) = 0$. Note: z-axis points up, $g=-9.8$.
Correct logic: $a(t) = -g - kv$. Terminal velocity is down.
Standard eq 13.96 derived for $g$ positive?
Let's use the coordinate system: $x(0)=50$, $x(t_{end})=0$. $g=9.8$.
Force $F = -mg + mkv$? Or drag opposes motion (up).
Eq 13.96: $x(t) = x_0 + \frac{g}{k}t \dots$ This grows positively.
Let's use standard form for falling: $z(t) = z_0 - \frac{g}{k}t + \frac{g}{k^2}(1 - e^{-kt})$.
$f(t) = 50 - 9.8t + 9.8(1 - e^{-t}) = 0$.
$f(t) = 59.8 - 9.8t - 9.8e^{-t} = 0$.

**2. Newton's Method**
$f(t) = 59.8 - 9.8t - 9.8e^{-t}$
$f'(t) = -9.8 + 9.8e^{-t} = 9.8(e^{-t} - 1)$
Iteration: $t_{n+1} = t_n - \frac{f(t_n)}{f'(t_n)}$.

**Guess $t_0 = 6$:**
$f(6) = 59.8 - 58.8 - 9.8(0.0025) \approx 1.0 - 0.02 = 0.98$
$f'(6) = 9.8(0.0025 - 1) \approx -9.77$
$t_1 = 6 - \frac{0.98}{-9.77} \approx 6 + 0.10 = 6.10$.

**Check $t_1 = 6.10$:**
$f(6.1) = 59.8 - 59.78 - 9.8(0.0022) \approx 0.02 - 0.02 \approx 0$.
Root is approximately **6.10 seconds**.
