### Answer 3.5.1

**Matrix:**
$$ A = \begin{bmatrix} 1 & 1 & 1 & 2 & 0 \\ 3 & 3 & 0 & 6 & 0 \end{bmatrix} $$

**a. Dimensions of Subspaces:**
Perform row reduction:
$R_2 \leftarrow R_2 - 3R_1$:
$$ \begin{bmatrix} 1 & 1 & 1 & 2 & 0 \\ 0 & 0 & -3 & 0 & 0 \end{bmatrix} $$
Pivots are in columns 1 and 3. Rank $r = 2$.
$m = 2$ (rows), $n = 5$ (columns).
* $dim(Row(A)) = r = 2$.
* $dim(Col(A)) = r = 2$.
* $dim(Null(A)) = n - r = 5 - 2 = 3$.
* $dim(Left\text{-}null(A)) = m - r = 2 - 2 = 0$.

**b. Decomposition:**
Vector $\mathbf{x} = (-2, 0, 1, 4, 1)^T$.
We want $\mathbf{x} = \mathbf{x}_R + \mathbf{x}_0$ where $\mathbf{x}_R \in Row(A)$ and $\mathbf{x}_0 \in Null(A)$.
Since $Row(A) \perp Null(A)$, this is an orthogonal decomposition.
$\mathbf{x}_R$ is the projection of $\mathbf{x}$ onto $Row(A)$.
Alternatively, solve $A\mathbf{x} = A(\mathbf{x}_R + \mathbf{x}_0) = A\mathbf{x}_R$.
Since $\mathbf{x}_R \in Row(A)$, $\mathbf{x}_R = A^T \mathbf{y}$.
So $A(A^T \mathbf{y}) = A\mathbf{x}$.
Calculate $A\mathbf{x}$:
$$ \begin{bmatrix} 1 & 1 & 1 & 2 & 0 \\ 3 & 3 & 0 & 6 & 0 \end{bmatrix} \begin{bmatrix} -2 \\ 0 \\ 1 \\ 4 \\ 1 \end{bmatrix} = \begin{bmatrix} -2+0+1+8+0 \\ -6+0+0+24+0 \end{bmatrix} = \begin{bmatrix} 7 \\ 18 \end{bmatrix} $$
Calculate $AA^T$:
$$ AA^T = \begin{bmatrix} 1 & 1 & 1 & 2 & 0 \\ 3 & 3 & 0 & 6 & 0 \end{bmatrix} \begin{bmatrix} 1 & 3 \\ 1 & 3 \\ 1 & 0 \\ 2 & 6 \\ 0 & 0 \end{bmatrix} = \begin{bmatrix} 7 & 18 \\ 18 & 54 \end{bmatrix} $$
Solve $\begin{bmatrix} 7 & 18 \\ 18 & 54 \end{bmatrix} \begin{bmatrix} y_1 \\ y_2 \end{bmatrix} = \begin{bmatrix} 7 \\ 18 \end{bmatrix}$.
Row reduction: $R_2 - (18/7)R_1 \dots$ easier: notice the RHS is exactly column 1.
So $y_1 = 1, y_2 = 0$.
Thus $\mathbf{x}_R = A^T \begin{bmatrix} 1 \\ 0 \end{bmatrix} = \text{Row 1 of A transposed} = (1, 1, 1, 2, 0)^T$.
Then $\mathbf{x}_0 = \mathbf{x} - \mathbf{x}_R = (-2, 0, 1, 4, 1) - (1, 1, 1, 2, 0) = (-3, -1, 0, 2, 1)^T$.

**Result:**
$\mathbf{x}_R = (1, 1, 1, 2, 0)^T$
$\mathbf{x}_0 = (-3, -1, 0, 2, 1)^T$