### Answer 3.5.23

**Formula:** $dim(U+V) = dim(U) + dim(V) - dim(U \cap V)$.
**Proof:**
Let basis for $U \cap V$ be $\{z_1, \dots, z_k\}$.
Extend to basis for $U$: $\{z_1, \dots, z_k, u_1, \dots, u_p\}$. ($dim(U) = k+p$).
Extend to basis for $V$: $\{z_1, \dots, z_k, v_1, \dots, v_q\}$. ($dim(V) = k+q$).
Claim: $B = \{z's, u's, v's\}$ is basis for $U+V$.
Span: Clear.
Independence: $\sum a z + \sum b u + \sum c v = 0$.
$\sum b u = - \sum a z - \sum c v$.
LHS $\in U$. RHS $\in V$ (since $z \in V$).
Thus LHS $\in U \cap V$.
$\sum b u = \sum d z$.
$\sum b u - \sum d z = 0$.
Since $\{u, z\}$ basis for U, $b=0$.
Similarly $c=0$, then $a=0$.
Count: $k + p + q = (k+p) + (k+q) - k = dim(U) + dim(V) - dim(U \cap V)$.