### Answer 6.2.12

**Proof:**
Using $A^{-1} = \frac{1}{det(A)} adj(A)$, we have $adj(A) = det(A) A^{-1}$.
Invert both sides:
$(adj(A))^{-1} = (det(A) A^{-1})^{-1}$.
$(adj(A))^{-1} = \frac{1}{det(A)} (A^{-1})^{-1} = \frac{1}{det(A)} A$.

Now consider $adj(A^{-1})$.
Formula: $adj(B) = det(B) B^{-1}$. Let $B = A^{-1}$.
$adj(A^{-1}) = det(A^{-1}) (A^{-1})^{-1}$.
Using $det(A^{-1}) = 1/det(A)$ and $(A^{-1})^{-1} = A$:
$adj(A^{-1}) = \frac{1}{det(A)} A$.

Since both expressions equal $\frac{1}{det(A)} A$, they are equal.