### Answer 6.1

We start with the identity $(e^{i\theta})^3 = e^{i(3\theta)}$.

**1. Expand the Left Side:**
Using $e^{i\theta} = \cos \theta + i \sin \theta$:
$$(e^{i\theta})^3 = (\cos \theta + i \sin \theta)^3$$
$$= \cos^3 \theta + 3 \cos^2 \theta (i \sin \theta) + 3 \cos \theta (i \sin \theta)^2 + (i \sin \theta)^3$$
$$= \cos^3 \theta + 3i \cos^2 \theta \sin \theta - 3 \cos \theta \sin^2 \theta - i \sin^3 \theta$$
Group real and imaginary parts:
$$= (\cos^3 \theta - 3 \cos \theta \sin^2 \theta) + i(3 \cos^2 \theta \sin \theta - \sin^3 \theta)$$

**2. Substitute $\sin^2 \theta = 1 - \cos^2 \theta$ into the Real Part:**
$$Re = \cos^3 \theta - 3 \cos \theta (1 - \cos^2 \theta)$$
$$= \cos^3 \theta - 3 \cos \theta + 3 \cos^3 \theta$$
$$= 4 \cos^3 \theta - 3 \cos \theta$$

**3. Expand the Right Side:**
$$e^{i(3\theta)} = \cos 3\theta + i \sin 3\theta$$

**4. Equate Real Parts:**
$$4 \cos^3 \theta - 3 \cos \theta = \cos 3\theta$$
