### Answer 6.7

**1. Cone Geometry:**
Apex at $(0, 0, h)$. Base at $z=0$ with radius $r$.
The radius at height $z$ is linear: $R(z) = r(1 - \frac{z}{h}) = \frac{r}{h}(h-z)$.
Implicit equation: $x^2 + y^2 = [R(z)]^2 \implies x^2 + y^2 = \frac{r^2}{h^2}(h-z)^2$.

**2. Substitute Ray $P(t) = S + tV$:**
$$(S_x + tV_x)^2 + (S_y + tV_y)^2 = \frac{r^2}{h^2}(h - (S_z + tV_z))^2$$

**3. Expand terms:**
Left Side (LHS):
$$(V_x^2 + V_y^2)t^2 + 2(S_x V_x + S_y V_y)t + (S_x^2 + S_y^2)$$

Right Side (RHS):
Let $k = r/h$.
$$k^2 [ (h - S_z) - tV_z ]^2 = k^2 [ V_z^2 t^2 - 2V_z(h-S_z)t + (h-S_z)^2 ]$$

**4. Form Polynomial $At^2 + Bt + C = 0$:**
$$A = V_x^2 + V_y^2 - k^2 V_z^2$$
$$B = 2(S_x V_x + S_y V_y) + 2k^2 V_z(h - S_z)$$
$$C = S_x^2 + S_y^2 - k^2 (h - S_z)^2$$
(where $k = r/h$).
