### Answer 1.3.12

**Given:** $P_0(1, -2, 4)$ and line $\mathbf{p} = (3, -2, 1) + t(2, 1, -3)$.

1.  **Find Vectors:**
    * Vector $\mathbf{u}$ from the line's direction: $(2, 1, -3)$.
    * Vector $\mathbf{v}$ connecting $P_0$ to a point on the line (e.g., $(3, -2, 1)$):
      $\mathbf{v} = (3, -2, 1) - (1, -2, 4) = (2, 0, -3)$.

2.  **Parametric Form:**
    $\mathbf{p} = P_0 + s\mathbf{u} + t\mathbf{v}$
    $\mathbf{p} = (1, -2, 4) + s(2, 1, -3) + t(2, 0, -3)$.

3.  **Nonparametric Form (Normal Vector):**
    $\mathbf{n} = \mathbf{u} \times \mathbf{v} = \begin{vmatrix} \mathbf{i} & \mathbf{j} & \mathbf{k} \\ 2 & 1 & -3 \\ 2 & 0 & -3 \end{vmatrix} = (-3, 0, -2)$.
    Equation: $-3(x-1) + 0(y+2) - 2(z-4) = 0$.
    $-3x - 2z + 11 = 0 \implies 3x + 2z = 11$.