### Answer 1.3.24

**Line:** $P_L = (3, -2, 6) + s_1(-3, 5, 7)$.
**Plane:** $P_P = (4, -2, 1) + s_2(-2, 1, 3) + t(1, 3, 2)$.

**Method:**
Convert plane to nonparametric form first.
$\mathbf{n} = (-2, 1, 3) \times (1, 3, 2) = (2-9, 3+4, -6-1) = (-7, 7, -7)$.
Divide by -7: $\mathbf{n} = (1, -1, 1)$.
Plane Eq: $1(x-4) - 1(y+2) + 1(z-1) = 0 \implies x - y + z = 7$.

**Substitute Line:**
$(3-3s_1) - (-2+5s_1) + (6+7s_1) = 7$.
$3 - 3s_1 + 2 - 5s_1 + 6 + 7s_1 = 7$.
$11 - s_1 = 7$.
$s_1 = 4$.

**Intersection Point:**
$(3-12, -2+20, 6+28) = (-9, 18, 34)$.