### Answer 1.3.13

**Given:** Origin $O(0,0,0)$ and line $\mathbf{p} = (3, -2, 1) + t(2, 1, -3)$.

1.  **Find Vectors:**
    * $\mathbf{u} = (2, 1, -3)$ (Line direction).
    * $\mathbf{v} = (3, -2, 1) - (0,0,0) = (3, -2, 1)$ (Vector to line start).

2.  **Parametric Form:**
    $\mathbf{p} = s(2, 1, -3) + t(3, -2, 1)$.

3.  **Nonparametric Form:**
    $\mathbf{n} = \mathbf{u} \times \mathbf{v} = \begin{vmatrix} \mathbf{i} & \mathbf{j} & \mathbf{k} \\ 2 & 1 & -3 \\ 3 & -2 & 1 \end{vmatrix} = (1-6, -9-2, -4-3) = (-5, -11, -7)$.
    Equation through origin: $-5x - 11y - 7z = 0$ (or $5x + 11y + 7z = 0$).