### Answer 5.6

We need to derive the third row of the projection matrix such that:
$$z_{ndc} = \frac{A z_{eye} + B}{-z_{eye}}$$
mapping $z_{eye} = -n \to z_{ndc} = 0$ and $z_{eye} = -f \to z_{ndc} = 1$.

**1. Near Plane Condition:**
$$\frac{A(-n) + B}{-(-n)} = 0$$
$$\frac{-An + B}{n} = 0 \implies -An + B = 0 \implies B = An$$

**2. Far Plane Condition:**
$$\frac{A(-f) + B}{-(-f)} = 1$$
$$\frac{-Af + B}{f} = 1 \implies -Af + B = f$$

**3. Solve System:**
Substitute $B = An$ into the second equation:
$$-Af + An = f$$
$$A(n - f) = f$$
$$A = \frac{f}{n - f}$$

Solve for B:
$$B = \frac{fn}{n - f}$$

**4. Result:**
The third row of the projection matrix (assuming $(x, y, z, w)$ column vectors and row-major layout, or simply the $z$-transform coefficients) is:
$$\langle 0, 0, \frac{f}{n - f}, \frac{fn}{n - f} \rangle$$
(Note: Standard OpenGL maps to $[-1, 1]$. This mapping to $[0, 1]$ corresponds to DirectX standards).
